@prefix : <https://uri.etsi.org/ngsi-ld/> .
@prefix owl: <http://www.w3.org/2002/07/owl#> .
@prefix rdf: <http://www.w3.org/1999/02/22-rdf-syntax-ns#> .
@prefix xml: <http://www.w3.org/XML/1998/namespace> .
@prefix xsd: <http://www.w3.org/2001/XMLSchema#> .
@prefix rdfs: <http://www.w3.org/2000/01/rdf-schema#> .
@prefix geojson: <https://purl.org/geojson/vocab#> .
@prefix smart: <https://smartdatamodels.org/> .
@prefix fiware: <https://uri.fiware.org/ns/data-models#> .
@prefix terms: <https://smart-data-models.github.io/data-models/terms.jsonld#/definitions/> .
@prefix definitions: <https://smart-data-models.github.io/data-models/common-schema.json#/definitions/> .
@prefix common: <https://smart-data-models.github.io/data-models/common-schema.json#/definitions/Location-Commons/properties/> .
@prefix saref: <https://w3id.org/def/saref#> .
@prefix saref4agri: <https://w3id.org/def/saref4agri#> .
@prefix goodrelations: <http://purl.org/goodrelations/v1#> .
@prefix purlterms: <http://purl.org/dc/terms/> .
@prefix schema: <https://schema.org/> .
@prefix ngsi-ld: <http://uri.etsi.org/ngsi-ld/> .
@prefix default: <https://uri.etsi.org/ngsi-ld/default-context/> .
@prefix building: <https://smartdatamodels.org/dataModel.Building/> .
@prefix energy: <https://smartdatamodels.org/dataModel.Energy/> .
@base <https://uri.etsi.org/ngsi-ld/> .

<https://uri.etsi.org/ngsi-ld/> rdf:type owl:Ontology .

#################################################################
#    Datatypes
#################################################################

### https://smart-data-models.github.io/data-models/terms.jsonld#/definitions/email
terms:email rdf:type rdfs:Datatype ;
            owl:onDatatype xsd:string ;
            rdfs:comment "idn-email. Property. Email address of owner" .

### https://smart-data-models.github.io/data-models/common-schema.json#/definitions/userAlias
definitions:userAlias rdf:type rdfs:Datatype ;
                      owl:onDatatype xsd:string ;
                      rdfs:comment "Property. An anonymous alias of a user" .

### https://smart-data-models.github.io/data-models/terms.jsonld#/definitions/tag
terms:tag rdf:type rdfs:Datatype ;
          owl:onDatatype xsd:string ;
          rdfs:comment "Property. Model:'https://schema.org/Text'. An optional text string used to qualify an item" .

### https://smart-data-models.github.io/data-models/common-schema.json#/definitions/timeInstant
definitions:timeInstant rdf:type rdfs:Datatype ;
                        owl:onDatatype xsd:dateTime ;
                        rdfs:comment "Property. Model:'https://schema.org/Datetime'. Timestamp of the payload . There can be production environments where the attribute type is equal to the `ISO8601` string. If so, it must be considered as a synonym of `DateTime`. This attribute is kept for backwards compatibility with old FIWARE reference implementations" .

### https://smartdatamodels.org/dateObserved
smart:dateObserved rdf:type rdfs:Datatype ;
                   owl:onDatatype xsd:dateTime ;
                   rdfs:comment "Property. Date of the observed entity defined by the user" .

### https://smart-data-models.github.io/data-models/common-schema.json#/definitions/dateYearLess
definitions:dateYearLess rdf:type rdfs:Datatype ;
                         owl:onDatatype xsd:string ;
                         owl:withRestrictions ( 
                                                 [ xsd:pattern "^--((0[13578]|1[02])-31|(0[1,3-9]|1[0-2])-30|(0\d|1[0-2])-([0-2]\d))$" ]
                                              ) .

### https://uri.etsi.org/ngsi-ld/default-context/touristType
default:touristType rdf:type rdfs:Datatype ;
                    owl:onDatatype xsd:string ;
                    rdfs:comment "Property. Model:'https://schema.org/Text'. Type of tourism depending on the segment and the motivation of the trip." .

### https://uri.etsi.org/ngsi-ld/default-context/isAccessibleForFree
default:isAccessibleForFree rdf:type rdfs:Datatype ;
                            owl:onDatatype xsd:boolean ;
                            rdfs:comment "Property. Model:'https://schema.org/isAccessibleForFree'. A flag to signal that the item, event, or place is accessible for free." .

### https://uri.etsi.org/ngsi-ld/default-context/publicAccess
default:publicAccess rdf:type rdfs:Datatype ;
                     owl:onDatatype xsd:boolean ;
                     rdfs:comment "Property. Model:'https://schema.org/publicAccess'. A flag to signal that the Place is open to public visitors. If this property is omitted there is no assumed default boolean value" .

### https://uri.etsi.org/ngsi-ld/default-context/availableLanguage
default:availableLanguage rdf:type rdfs:Datatype ;
                          owl:onDatatype rdf:List ;
                          rdfs:comment "Property. Model:''. A language someone may use with or at the item, service or place. Please use one of the language codes from the IETF BCP 47 standard. " .

### https://uri.etsi.org/ngsi-ld/default-context/video
default:video rdf:type rdfs:Datatype ;
              owl:onDatatype xsd:anyURI ;
              rdfs:comment "Property. Model:'https://schema.org/URL'. Url with video related to the item" .

#################################################################
#    Classes
#################################################################

### https://uri.etsi.org/ngsi-ld/Entity
:Entity rdf:type owl:Class ;
        owl:disjointWith :Property ,
                         :Relationship ,
                         :Value .


### https://uri.etsi.org/ngsi-ld/Geometry
:Geometry rdf:type owl:Class ;
          rdfs:subClassOf :Value .


### https://uri.etsi.org/ngsi-ld/LanguageMap
:LanguageMap rdf:type owl:Class ;
             rdfs:subClassOf :Value .


### https://uri.etsi.org/ngsi-ld/LineString
:LineString rdf:type owl:Class ;
            rdfs:subClassOf :Geometry .


### https://uri.etsi.org/ngsi-ld/Point
:Point rdf:type owl:Class ;
       rdfs:subClassOf :Geometry .


### https://uri.etsi.org/ngsi-ld/MultiPoint
:MultiPoint rdf:type owl:Class ;
            rdfs:subClassOf :Geometry .


### https://uri.etsi.org/ngsi-ld/Polygon
:Polygon rdf:type owl:Class ;
         rdfs:subClassOf :Geometry .


### https://uri.etsi.org/ngsi-ld/MultiPolygon
:MultiPolygon rdf:type owl:Class ;
              rdfs:subClassOf :Geometry .


### https://uri.etsi.org/ngsi-ld/Property
:Property rdf:type owl:Class ;
          owl:disjointWith :Relationship .


### https://uri.etsi.org/ngsi-ld/Relationship
:Relationship rdf:type owl:Class ;
              owl:disjointWith :Value .


### https://uri.etsi.org/ngsi-ld/Value
:Value rdf:type owl:Class .


### https://smartdatamodels.org/dataModel.Building/BuildingOperation
building:BuildingOperation rdf:type owl:Class ;
                           rdfs:subClassOf :Entity ;
                           rdfs:subClassOf [ rdf:type owl:Restriction ;
                                             owl:onProperty building:refBuilding ;
                                             owl:minCardinalityQ "1"^^xsd:nonNegativeInteger
                                           ] ;
                           rdfs:subClassOf [ rdf:type owl:Restriction ;
                                             owl:onProperty smart:startDate ;
                                             owl:minCardinalityQ "1"^^xsd:nonNegativeInteger
                                           ] ;
                           rdfs:subClassOf [ rdf:type owl:Restriction ;
                                             owl:onProperty smart:endDate ;
                                             owl:minCardinalityQ "1"^^xsd:nonNegativeInteger
                                           ] .


### https://smartdatamodels.org/dataModel.Building/Building
building:Building rdf:type owl:Class ;
                  rdfs:subClassOf :Entity ;
                  rdfs:subClassOf [ rdf:type owl:Restriction ;
                                    owl:onProperty building:category ;
                                    owl:minCardinalityQ "1"^^xsd:nonNegativeInteger
                                  ] ;
                  rdfs:subClassOf [ rdf:type owl:Restriction ;
                                    owl:onProperty smart:address ;
                                    owl:minCardinalityQ "1"^^xsd:nonNegativeInteger
                                  ] .


### https://uri.etsi.org/ngsi-ld/default-context/addressType
default:addressType rdf:type owl:Class ;
                    rdfs:subClassOf :Value ;
                    rdfs:comment "Value. The mailing address. Model:'https://schema.org/address'" .


### https://smartdatamodels.org/dataModel.Building/VibrationsObserved
building:VibrationsObserved rdf:type owl:Class ;
                            rdfs:subClassOf :Entity ;
                            rdfs:subClassOf [ rdf:type owl:Restriction ;
                                              owl:onProperty smart:dateObserved ;
                                              owl:minCardinalityQ "1"^^xsd:nonNegativeInteger
                                            ] ;
                            rdfs:subClassOf [ rdf:type owl:Restriction ;
                                              owl:onProperty building:accelerationMeasured ;
                                              owl:minCardinalityQ "1"^^xsd:nonNegativeInteger
                                            ] .


### https://smartdatamodels.org/dataModel.Energy/ACMeasurement
energy:ACMeasurement rdf:type owl:Class ;
                     rdfs:subClassOf :Entity ;
                     rdfs:subClassOf [ rdf:type owl:Restriction ;
                                       owl:onProperty ngsi-ld:location ;
                                       owl:minCardinalityQ "1"^^xsd:nonNegativeInteger
                                     ] ;
                     rdfs:subClassOf [ rdf:type owl:Restriction ;
                                       owl:onProperty smart:dateObserved ;
                                       owl:minCardinalityQ "1"^^xsd:nonNegativeInteger
                                     ] ;
                     rdfs:subClassOf [ rdf:type owl:Restriction ;
                                       owl:onProperty energy:phaseType ;
                                       owl:minCardinalityQ "1"^^xsd:nonNegativeInteger
                                     ] .


### https://uri.etsi.org/ngsi-ld/default-context/activeEnergyImportType
default:activeEnergyImportType rdf:type owl:Class ;
                               rdfs:subClassOf :Value ;
                               rdfs:comment "Value. Model:'https://schema.org/StructuredValue'. Active energy imported i.e. consumed per phase. The unit code (text) is given using the [UN/CEFACT Common Codes](http://wiki.goodrelations-vocabulary.org/Documentation/UN/CEFACT_Common_Codes). Units:'kilowatt hour'" .


### https://uri.etsi.org/ngsi-ld/default-context/reactiveEnergyImportType
default:reactiveEnergyImportType rdf:type owl:Class ;
                                 rdfs:subClassOf :Value ;
                                 rdfs:comment "Value. Model:'https://schema.org/StructuredValue'. Fundamental frequency reactive energy imported i.e. consumed per phase. The unit code (text) is given using the [UN/CEFACT Common Codes](http://wiki.goodrelations-vocabulary.org/Documentation/UN/CEFACT_Common_Codes). Units:'kilovolt-ampere-reactive-hour'" .


### https://uri.etsi.org/ngsi-ld/default-context/apparentEnergyImportType
default:apparentEnergyImportType rdf:type owl:Class ;
                                 rdfs:subClassOf :Value ;
                                 rdfs:comment "Value. Model:'https://schema.org/StructuredValue'. Apparent energy imported i.e. consumed per phase. The unit code (text) is given using the [UN/CEFACT Common Codes](http://wiki.goodrelations-vocabulary.org/Documentation/UN/CEFACT_Common_Codes). Units:'kilovolt-ampere-hour'" .


### https://uri.etsi.org/ngsi-ld/default-context/activeEnergyExportType
default:activeEnergyExportType rdf:type owl:Class ;
                               rdfs:subClassOf :Value ;
                               rdfs:comment "Value. Model:'https://schema.org/StructuredValue'. Active energy exported per phase. The unit code (text) is given using the [UN/CEFACT Common Codes](http://wiki.goodrelations-vocabulary.org/Documentation/UN/CEFACT_Common_Codes). Units:'kilowatt hour'" .


### https://uri.etsi.org/ngsi-ld/default-context/reactiveEnergyExportType
default:reactiveEnergyExportType rdf:type owl:Class ;
                                 rdfs:subClassOf :Value ;
                                 rdfs:comment "Value. Model:'https://schema.org/StructuredValue'. Fundamental frequency reactive energy exported per phase. The unit code (text) is given using the [UN/CEFACT Common Codes](http://wiki.goodrelations-vocabulary.org/Documentation/UN/CEFACT_Common_Codes). Units:'kilovolt-ampere-reactive-hour'" .


### https://uri.etsi.org/ngsi-ld/default-context/apparentEnergyExportType
default:apparentEnergyExportType rdf:type owl:Class ;
                                 rdfs:subClassOf :Value ;
                                 rdfs:comment "Value. Model:'https://schema.org/StructuredValue'. Apparent energy exported per phase. The unit code (text) is given using the [UN/CEFACT Common Codes](http://wiki.goodrelations-vocabulary.org/Documentation/UN/CEFACT_Common_Codes). Units:'kilovolt-ampere-hour'" .


### https://uri.etsi.org/ngsi-ld/default-context/activePowerType
default:activePowerType rdf:type owl:Class ;
                        rdfs:subClassOf :Value ;
                        rdfs:comment "Value. Model:'https://schema.org/StructuredValue'. Active power consumed per phase. The unit code (text) is given using the [UN/CEFACT Common Codes](http://wiki.goodrelations-vocabulary.org/Documentation/UN/CEFACT_Common_Codes). Units:'Watt'" .


### https://uri.etsi.org/ngsi-ld/default-context/reactivePowerType
default:reactivePowerType rdf:type owl:Class ;
                          rdfs:subClassOf :Value ;
                          rdfs:comment "Value. Model:'https://schema.org/StructuredValue'. Fundamental frequency reactive power. The unit code (text) is given using the [UN/CEFACT Common Codes](http://wiki.goodrelations-vocabulary.org/Documentation/UN/CEFACT_Common_Codes). Units:'volts-ampere-reactive'" .


### https://uri.etsi.org/ngsi-ld/default-context/apparentPowerType
default:apparentPowerType rdf:type owl:Class ;
                          rdfs:subClassOf :Value ;
                          rdfs:comment "Value. Model:'https://schema.org/StructuredValue'. Apparent power consumed per phase. The unit code (text) is given using the [UN/CEFACT Common Codes](http://wiki.goodrelations-vocabulary.org/Documentation/UN/CEFACT_Common_Codes). Units:'Watt'" .


### https://uri.etsi.org/ngsi-ld/default-context/powerFactorType
default:powerFactorType rdf:type owl:Class ;
                        rdfs:subClassOf :Value ;
                        rdfs:comment "Value. Model:'https://schema.org/StructuredValue'. Power factor for each phase" .


### https://uri.etsi.org/ngsi-ld/default-context/displacementPowerFactorType
default:displacementPowerFactorType rdf:type owl:Class ;
                                    rdfs:subClassOf :Value ;
                                    rdfs:comment "Value. Model:'https://schema.org/StructuredValue'. Displacement power factor for each phase. The quantity is based on the fundamental frequency of the system" .


### https://uri.etsi.org/ngsi-ld/default-context/currentType
default:currentType rdf:type owl:Class ;
                    rdfs:subClassOf :Value ;
                    rdfs:comment "Value. Model:'https://schema.org/StructuredValue'. Electrical current. The unit code (text) is given using the [UN/CEFACT Common Codes](http://wiki.goodrelations-vocabulary.org/Documentation/UN/CEFACT_Common_Codes). Units:'Ampere'" .


### https://uri.etsi.org/ngsi-ld/default-context/phaseVoltageType
default:phaseVoltageType rdf:type owl:Class ;
                         rdfs:subClassOf :Value ;
                         rdfs:comment "Value. Model:'https://schema.org/StructuredValue'. The voltage between each phase and neutral conductor. The unit code (text) is given using the [UN/CEFACT Common Codes](http://wiki.goodrelations-vocabulary.org/Documentation/UN/CEFACT_Common_Codes). Units:'Volts'" .


### https://uri.etsi.org/ngsi-ld/default-context/thdVoltageType
default:thdVoltageType rdf:type owl:Class ;
                       rdfs:subClassOf :Value ;
                       rdfs:comment "Value. Model:'https://schema.org/StructuredValue'. Total harmonic distortion of voltage for each phase" .


### https://uri.etsi.org/ngsi-ld/default-context/thdCurrentType
default:thdCurrentType rdf:type owl:Class ;
                       rdfs:subClassOf :Value ;
                       rdfs:comment "Value. Model:'https://schema.org/StructuredValue'. Total harmonic distortion of current for each phase" .


### https://uri.etsi.org/ngsi-ld/default-context/phaseToPhaseVoltageType
default:phaseToPhaseVoltageType rdf:type owl:Class ;
                                rdfs:subClassOf :Value ;
                                rdfs:comment "Value. Model:'https://schema.org/StructuredValue'. Voltage between phases. The unit code (text) is given using the [UN/CEFACT Common Codes](http://wiki.goodrelations-vocabulary.org/Documentation/UN/CEFACT_Common_Codes). Units:'Volts'" .


### https://smartdatamodels.org/dataModel.Energy/InverterDevice
energy:InverterDevice rdf:type owl:Class ;
                      rdfs:subClassOf :Entity ;
                      rdfs:subClassOf [ rdf:type owl:Restriction ;
                                        owl:onProperty ngsi-ld:location ;
                                        owl:minCardinalityQ "1"^^xsd:nonNegativeInteger
                                      ] ;
                      rdfs:subClassOf [ rdf:type owl:Restriction ;
                                        owl:onProperty energy:dateLastReported ;
                                        owl:minCardinalityQ "1"^^xsd:nonNegativeInteger
                                      ] ;
                      rdfs:subClassOf [ rdf:type owl:Restriction ;
                                        owl:onProperty energy:phaseType ;
                                        owl:minCardinalityQ "1"^^xsd:nonNegativeInteger
                                      ] .


### https://uri.etsi.org/ngsi-ld/default-context/dimensionType
default:dimensionType rdf:type owl:Class ;
                      rdfs:subClassOf :Value ;
                      rdfs:comment "Value. External dimension of a Panel. The format is structured by a sub-property of 3 items. The unit code (text) is given using the [UN/CEFACT Common Codes](http://wiki.goodrelations-vocabulary.org/Documentation/UN/CEFACT_Common_Codes). For instance, **CMT** represents Centimeter. Units:'Centimeters'" .


### https://uri.etsi.org/ngsi-ld/default-context/operatingTemperatureType
default:operatingTemperatureType rdf:type owl:Class ;
                                 rdfs:subClassOf :Value ;
                                 rdfs:comment "Value. Ambient operating temperature range. This is the minimum and maximum resistance to cold and heat. The format is structured by a sub-property of 2 items. The unit code (text) is given using the [UN/CEFACT Common Codes](http://wiki.goodrelations-vocabulary.org/Documentation/UN/CEFACT_Common_Codes). For instance, **CEL** represents Degree Celsius" .


### https://uri.etsi.org/ngsi-ld/default-context/operatingAirHumidityType
default:operatingAirHumidityType rdf:type owl:Class ;
                                 rdfs:subClassOf :Value ;
                                 rdfs:comment "Value. Ambient operating Air Humidity range. The format is structured by a sub-property of 2 items. The unit code (text) is given using the [UN/CEFACT Common Codes](http://wiki.goodrelations-vocabulary.org/Documentation/UN/CEFACT_Common_Codes). For instance, **P1** represents Percent" .


### https://uri.etsi.org/ngsi-ld/default-context/operatingVoltageDCType
default:operatingVoltageDCType rdf:type owl:Class ;
                               rdfs:subClassOf :Value ;
                               rdfs:comment "Value. Minimum and Maximum voltage allowed. The format is structured by a sub-property of 2 items. The unit code (text) is given using the [UN/CEFACT Common Codes](http://wiki.goodrelations-vocabulary.org/Documentation/UN/CEFACT_Common_Codes). For instance, **VLT** represents Volt.. Model:'https://schema.org/Number'. Units:'Volt'" .


### https://uri.etsi.org/ngsi-ld/default-context/operatingAmpereDCType
default:operatingAmpereDCType rdf:type owl:Class ;
                              rdfs:subClassOf :Value ;
                              rdfs:comment "Value. Minimum and Maximum Ampere allowed.. The format is structured by a sub-property of 2 items. The unit code (text) is given using the [UN/CEFACT Common Codes](http://wiki.goodrelations-vocabulary.org/Documentation/UN/CEFACT_Common_Codes). For instance, **AMP** represents Ampere. Model:'https://schema.org/Number'. Units:'Ampere'" .


### https://uri.etsi.org/ngsi-ld/default-context/operatingFrequencyDCType
default:operatingFrequencyDCType rdf:type owl:Class ;
                                 rdfs:subClassOf :Value ;
                                 rdfs:comment "Value. Minimum and Maximum Frequency allowed. The format is structured by a sub-property of 2 items. The unit code (text) is given using the [UN/CEFACT Common Codes](http://wiki.goodrelations-vocabulary.org/Documentation/UN/CEFACT_Common_Codes). For instance, **HTZ** represents Hertz. Model:'https://schema.org/Number'. Units:'Hertz'" .


### https://uri.etsi.org/ngsi-ld/default-context/mPPTPVVoltageDCType
default:mPPTPVVoltageDCType rdf:type owl:Class ;
                            rdfs:subClassOf :Value ;
                            rdfs:comment "Value. Minimum and Maximum Photo-voltaic voltage range, MPPT allowed. The format is structured by a sub-property of 2 items. The unit code (text) is given using the [UN/CEFACT Common Codes](http://wiki.goodrelations-vocabulary.org/Documentation/UN/CEFACT_Common_Codes). For instance, **VLT** represents Volt. Model:'https://schema.org/Number'. Units:'Volt'" .


### https://uri.etsi.org/ngsi-ld/default-context/operatingVoltageACType
default:operatingVoltageACType rdf:type owl:Class ;
                               rdfs:subClassOf :Value ;
                               rdfs:comment "Value. Minimum and Maximum voltage allowed. The format is structured by a sub-property of 2 items. The unit code (text) is given using the [UN/CEFACT Common Codes](http://wiki.goodrelations-vocabulary.org/Documentation/UN/CEFACT_Common_Codes). For instance, **VLT** represents Volt. Units:'Volt'. Model:'http://schema.org/StructuredValue'" .


### https://uri.etsi.org/ngsi-ld/default-context/operatingAmpereACType
default:operatingAmpereACType rdf:type owl:Class ;
                              rdfs:subClassOf :Value ;
                              rdfs:comment "Value. Minimum and Maximum Ampere allowed.. The format is structured by a sub-property of 2 items. The unit code (text) is given using the [UN/CEFACT Common Codes](http://wiki.goodrelations-vocabulary.org/Documentation/UN/CEFACT_Common_Codes). For instance, **AMP** represents Ampere. Model:'http://schema.org/Number'. Units:'Ampere'" .


### https://uri.etsi.org/ngsi-ld/default-context/operatingFrequencyACType
default:operatingFrequencyACType rdf:type owl:Class ;
                                 rdfs:subClassOf :Value ;
                                 rdfs:comment "Value. Minimum and Maximum Frequency allowed. The format is structured by a sub-property of 2 items. The unit code (text) is given using the [UN/CEFACT Common Codes](http://wiki.goodrelations-vocabulary.org/Documentation/UN/CEFACT_Common_Codes). For instance, **HTZ** represents Hertz. Units:'Volt'. Model:'http://schema.org/StructuredValue'. Units:'Hertz'" .


### https://uri.etsi.org/ngsi-ld/default-context/moduleYieldRateType
default:moduleYieldRateType rdf:type owl:Class ;
                            rdfs:subClassOf :Value ;
                            rdfs:comment "Value. Yield Rate of the Device. The format is structured by a sub-property of 2 items (European Standard - Manufacturer Standard). The unit code (text) is given using the [UN/CEFACT Common Codes](http://wiki.goodrelations-vocabulary.org/Documentation/UN/CEFACT_Common_Codes). For instance, **P1** represents Percent. Model:'http://schema.org/StructuredValue'" .


### https://smartdatamodels.org/dataModel.Energy/TechnicalCabinetDevice
energy:TechnicalCabinetDevice rdf:type owl:Class ;
                              rdfs:subClassOf :Entity ;
                              rdfs:subClassOf [ rdf:type owl:Restriction ;
                                                owl:onProperty ngsi-ld:location ;
                                                owl:minCardinalityQ "1"^^xsd:nonNegativeInteger
                                              ] ;
                              rdfs:subClassOf [ rdf:type owl:Restriction ;
                                                owl:onProperty energy:dateLastReported ;
                                                owl:minCardinalityQ "1"^^xsd:nonNegativeInteger
                                              ] ;
                              rdfs:subClassOf [ rdf:type owl:Restriction ;
                                                owl:onProperty energy:typeOfUse ;
                                                owl:minCardinalityQ "1"^^xsd:nonNegativeInteger
                                              ] ;
                              rdfs:subClassOf [ rdf:type owl:Restriction ;
                                                owl:onProperty energy:dimension ;
                                                owl:minCardinalityQ "1"^^xsd:nonNegativeInteger
                                              ] .


### https://uri.etsi.org/ngsi-ld/default-context/internalDimensionType
default:internalDimensionType rdf:type owl:Class ;
                              rdfs:subClassOf :Value ;
                              rdfs:comment "Value. Internal dimension corresponding to the place to work inside the technical cabinet. The format is structured by a sub-property of 3 items. The unit code (text) of measurement  is given using the [UN/CEFACT Common Codes](http://wiki.goodrelations-vocabulary.org/Documentation/UN/CEFACT_Common_Codes). For instance, **CMT** represents Centimeter. Model:'https://schema.org/StructuredValue'" .


### https://smartdatamodels.org/dataModel.Energy/ThreePhaseAcMeasurement
energy:ThreePhaseAcMeasurement rdf:type owl:Class ;
                               rdfs:subClassOf :Entity .


#################################################################
#    Object Properties
#################################################################

###  https://uri.etsi.org/ngsi-ld/GeoProperty
:GeoProperty rdf:type owl:ObjectProperty ;
             rdfs:subPropertyOf :Property ;
             rdfs:range :Geometry .

###  https://uri.etsi.org/ngsi-ld/LanguageProperty
:LanguageProperty rdf:type owl:ObjectProperty ;
                  rdfs:subPropertyOf :Property ;
                  rdfs:range :LanguageMap .

###  https://uri.etsi.org/ngsi-ld/Property
:Property rdf:type owl:ObjectProperty ;
          rdfs:domain [ rdf:type owl:Class ;
                        owl:unionOf ( :Entity
                                      :Property
                                      :Relationship
                                    )
                      ] ;
          rdfs:range [ rdf:type owl:Class ;
                       owl:unionOf ( :Property
                                     :Value
                                   )
                     ] .

###  https://uri.etsi.org/ngsi-ld/Relationship
:Relationship rdf:type owl:ObjectProperty ;
              rdfs:domain [ rdf:type owl:Class ;
                            owl:unionOf ( :Entity
                                          :Property
                                          :Relationship
                                        )
                          ] ;
              rdfs:range [ rdf:type owl:Class ;
                           owl:unionOf ( :Entity
                                         :Relationship
                                       )
                         ] .

###  https://uri.etsi.org/ngsi-ld/hasObject
:hasObject rdf:type owl:ObjectProperty ;
           rdfs:domain :Relationship ;
           rdfs:range :Entity .

###  https://uri.etsi.org/ngsi-ld/location
:location rdf:type owl:ObjectProperty ;
          rdfs:subPropertyOf :GeoProperty .

###  https://uri.etsi.org/ngsi-ld/observationSpace
:observationSpace rdf:type owl:ObjectProperty ;
                  rdfs:subPropertyOf :GeoProperty .

###  https://uri.etsi.org/ngsi-ld/operationSpace
:operationSpace rdf:type owl:ObjectProperty ;
                rdfs:subPropertyOf :GeoProperty .

###  https://smartdatamodels.org/owner
smart:owner rdf:type owl:ObjectProperty ;
            rdfs:subPropertyOf :Relationship ;
            rdfs:domain [ rdf:type owl:Class ;
                          owl:unionOf ( building:BuildingOperation
                                        building:Building
                                        building:VibrationsObserved
                                        energy:ACMeasurement
                                        energy:InverterDevice
                                        energy:TechnicalCabinetDevice
                                        energy:ThreePhaseAcMeasurement
                                      )
                        ] ;
            rdfs:range :Entity ;
            rdfs:comment "Property. A List containing a JSON encoded sequence of characters referencing the unique Ids of the owner(s)" .

###  https://smartdatamodels.org/dataModel.Building/refBuilding
building:refBuilding rdf:type owl:ObjectProperty ;
                     rdfs:subPropertyOf :Relationship ;
                     rdfs:domain building:BuildingOperation ;
                     rdfs:range :Entity ;
                     rdfs:comment "Relationship. Model:'https://schema.org/URL'. Building reference where the operation is performed" .

###  https://smartdatamodels.org/dataModel.Building/refOperator
building:refOperator rdf:type owl:ObjectProperty ;
                     rdfs:subPropertyOf :Relationship ;
                     rdfs:domain building:BuildingOperation ;
                     rdfs:range :Entity ;
                     rdfs:comment "Relationship. Model:'https://schema.org/URL'. Reference to the Operator doing the operation on the building" .

###  https://smartdatamodels.org/dataModel.Building/refRelatedBuildingOperation
building:refRelatedBuildingOperation rdf:type owl:ObjectProperty ;
                                     rdfs:subPropertyOf :Relationship ;
                                     rdfs:domain building:BuildingOperation ;
                                     rdfs:range :Entity ;
                                     rdfs:comment "Relationship. Reference to other building operations when in sequence" .

###  https://smartdatamodels.org/dataModel.Building/refRelatedDeviceOperation
building:refRelatedDeviceOperation rdf:type owl:ObjectProperty ;
                                   rdfs:subPropertyOf :Relationship ;
                                   rdfs:domain building:BuildingOperation ;
                                   rdfs:range :Entity ;
                                   rdfs:comment "Relationship. Devices related to the current operation. Model:'https://schema.org/URL'. A list of references to an entity of type Device" .

###  https://smartdatamodels.org/address
smart:address rdf:type owl:ObjectProperty ;
              rdfs:subPropertyOf :Property ;
              rdfs:domain [ rdf:type owl:Class ;
                            owl:unionOf ( building:Building
                                          building:VibrationsObserved
                                          energy:ACMeasurement
                                          energy:InverterDevice
                                          energy:TechnicalCabinetDevice
                                          energy:ThreePhaseAcMeasurement
                                        )
                          ] ;
              rdfs:range default:addressType ;
              rdfs:comment "Property. The mailing address. Model:'https://schema.org/address'" .

###  https://smartdatamodels.org/dataModel.Building/occupier
building:occupier rdf:type owl:ObjectProperty ;
                  rdfs:subPropertyOf :Relationship ;
                  rdfs:domain building:Building ;
                  rdfs:range :Entity ;
                  rdfs:comment "Relationship. Person or entity using the building. Model:'https://schema.org/URL'" .

###  https://uri.etsi.org/ngsi-ld/default-context/mapUrl
default:mapUrl rdf:type owl:ObjectProperty ;
               rdfs:subPropertyOf :Relationship ;
               rdfs:domain building:Building ;
               rdfs:range :Entity ;
               rdfs:comment "Relationship. Reference to the map containing the building" .

###  https://smartdatamodels.org/dataModel.Energy/refDevice
energy:refDevice rdf:type owl:ObjectProperty ;
                 rdfs:subPropertyOf :Relationship ;
                 rdfs:domain [ rdf:type owl:Class ;
                               owl:unionOf ( energy:ACMeasurement
                                             energy:InverterDevice
                                             energy:TechnicalCabinetDevice
                                             energy:ThreePhaseAcMeasurement
                                           )
                             ] ;
                 rdfs:range :Entity ;
                 rdfs:comment "Relationship. Device(s) used to obtain the measurement" .

###  https://smartdatamodels.org/dataModel.Energy/refTargetDevice
energy:refTargetDevice rdf:type owl:ObjectProperty ;
                       rdfs:subPropertyOf :Relationship ;
                       rdfs:domain [ rdf:type owl:Class ;
                                     owl:unionOf ( energy:ACMeasurement
                                                   energy:ThreePhaseAcMeasurement
                                                 )
                                   ] ;
                       rdfs:range :Entity ;
                       rdfs:comment "Relationship. Device(s) for which the measurement was taken" .

###  https://smartdatamodels.org/dataModel.Energy/activeEnergyImport
energy:activeEnergyImport rdf:type owl:ObjectProperty ;
                          rdfs:subPropertyOf :Property ;
                          rdfs:domain [ rdf:type owl:Class ;
                                        owl:unionOf ( energy:ACMeasurement
                                                      energy:ThreePhaseAcMeasurement
                                                    )
                                      ] ;
                          rdfs:range default:activeEnergyImportType ;
                          rdfs:comment "Property. Model:'http://schema.org/StructuredValue'. Units:'kilowatt hour (kWh)'. Active energy imported i.e. consumed per Line since the metering start date. The actual values will be conveyed by subproperties which names will be equal to the name of each of the alternating current phases: L1, L2, L3" .

###  https://smartdatamodels.org/dataModel.Energy/reactiveEnergyImport
energy:reactiveEnergyImport rdf:type owl:ObjectProperty ;
                            rdfs:subPropertyOf :Property ;
                            rdfs:domain [ rdf:type owl:Class ;
                                          owl:unionOf ( energy:ACMeasurement
                                                        energy:ThreePhaseAcMeasurement
                                                      )
                                        ] ;
                            rdfs:range default:reactiveEnergyImportType ;
                            rdfs:comment "Property. Model:'http://schema.org/StructuredValue'. Units:'kilovolt-ampere-reactive-hour (kVArh)'. Fundamental frequency reactive energy imported i.e. consumed per phase since the metering start date. The actual values will be conveyed by subproperties which names will be equal to the name of each of the alternating current phases: L1, L2, L3" .

###  https://smartdatamodels.org/dataModel.Energy/apparentEnergyImport
energy:apparentEnergyImport rdf:type owl:ObjectProperty ;
                            rdfs:subPropertyOf :Property ;
                            rdfs:domain [ rdf:type owl:Class ;
                                          owl:unionOf ( energy:ACMeasurement
                                                        energy:ThreePhaseAcMeasurement
                                                      )
                                        ] ;
                            rdfs:range default:apparentEnergyImportType ;
                            rdfs:comment "Property. Model:'http://schema.org/StructuredValue'. Units:'kilovolt-ampere-hour (kVAh)'. Apparent energy imported i.e. consumed per phase since the metering start date. The actual values will be conveyed by subproperties which names will be equal to the name of each of the alternating current phases: L1, L2, L3" .

###  https://smartdatamodels.org/dataModel.Energy/activeEnergyExport
energy:activeEnergyExport rdf:type owl:ObjectProperty ;
                          rdfs:subPropertyOf :Property ;
                          rdfs:domain [ rdf:type owl:Class ;
                                        owl:unionOf ( energy:ACMeasurement
                                                      energy:ThreePhaseAcMeasurement
                                                    )
                                      ] ;
                          rdfs:range default:activeEnergyExportType ;
                          rdfs:comment "Property. Model:'http://schema.org/StructuredValue'. Units:'kilowatt hour (kWh)'. Active energy exported per phase since the metering start date. The actual values will be conveyed by subproperties which names will be equal to the name of each of the alternating current phases: L1, L2, L3" .

###  https://smartdatamodels.org/dataModel.Energy/reactiveEnergyExport
energy:reactiveEnergyExport rdf:type owl:ObjectProperty ;
                            rdfs:subPropertyOf :Property ;
                            rdfs:domain [ rdf:type owl:Class ;
                                          owl:unionOf ( energy:ACMeasurement
                                                        energy:ThreePhaseAcMeasurement
                                                      )
                                        ] ;
                            rdfs:range default:reactiveEnergyExportType ;
                            rdfs:comment "Property. Model:'http://schema.org/StructuredValue'. Units:'kilovolt-ampere-reactive-hour (kVArh)'. Fundamental frequency reactive energy exported per phase since the metering start date. The actual values will be conveyed by subproperties which names will be equal to the name of each of the alternating current phases: L1, L2, L3" .

###  https://smartdatamodels.org/dataModel.Energy/apparentEnergyExport
energy:apparentEnergyExport rdf:type owl:ObjectProperty ;
                            rdfs:subPropertyOf :Property ;
                            rdfs:domain [ rdf:type owl:Class ;
                                          owl:unionOf ( energy:ACMeasurement
                                                        energy:ThreePhaseAcMeasurement
                                                      )
                                        ] ;
                            rdfs:range default:apparentEnergyExportType ;
                            rdfs:comment "Property. Model:'http://schema.org/StructuredValue'. Units:'kilovolt-ampere-hour (kVAh)'. Apparent energy exported per phase since the metering start date. The actual values will be conveyed by subproperties which names will be equal to the name of each of the alternating current phases: L1, L2, L3" .

###  https://smartdatamodels.org/dataModel.Energy/activePower
energy:activePower rdf:type owl:ObjectProperty ;
                   rdfs:subPropertyOf :Property ;
                   rdfs:domain [ rdf:type owl:Class ;
                                 owl:unionOf ( energy:ACMeasurement
                                               energy:ThreePhaseAcMeasurement
                                             )
                               ] ;
                   rdfs:range default:activePowerType ;
                   rdfs:comment "Property. Model:'http://schema.org/StructuredValue'. Units:'watt (W)'.Active power consumed per phase. The actual values will beconveyed by subproperties which names will be equal to the name of each of the alternating current phases: L1, L2, L3. " .

###  https://smartdatamodels.org/dataModel.Energy/reactivePower
energy:reactivePower rdf:type owl:ObjectProperty ;
                     rdfs:subPropertyOf :Property ;
                     rdfs:domain [ rdf:type owl:Class ;
                                   owl:unionOf ( energy:ACMeasurement
                                                 energy:ThreePhaseAcMeasurement
                                               )
                                 ] ;
                     rdfs:range default:reactivePowerType ;
                     rdfs:comment "Property. Model:'http://schema.org/StructuredValue'. Units:'volts-ampere-reactive (VAr)'. Fundamental frequency reactive power. The actual values will be conveyed by subproperties whose names will be equal to the name of each of the alternating current phases: L1, L2, L3" .

###  https://smartdatamodels.org/dataModel.Energy/apparentPower
energy:apparentPower rdf:type owl:ObjectProperty ;
                     rdfs:subPropertyOf :Property ;
                     rdfs:domain [ rdf:type owl:Class ;
                                   owl:unionOf ( energy:ACMeasurement
                                                 energy:ThreePhaseAcMeasurement
                                               )
                                 ] ;
                     rdfs:range default:apparentPowerType ;
                     rdfs:comment "Property. Model:'http://schema.org/StructuredValue'. Units:'volt-ampere (VA)'. Apparent power consumed per phase. The actual values will be conveyed by subproperties which names will be equal to the name of each of the alternating current phases: L1, L2, L3" .

###  https://smartdatamodels.org/dataModel.Energy/powerFactor
energy:powerFactor rdf:type owl:ObjectProperty ;
                   rdfs:subPropertyOf :Property ;
                   rdfs:domain [ rdf:type owl:Class ;
                                 owl:unionOf ( energy:ACMeasurement
                                               energy:ThreePhaseAcMeasurement
                                             )
                               ] ;
                   rdfs:range default:powerFactorType ;
                   rdfs:comment "Property. Model:'http://schema.org/StructuredValue'. Units:'-1 to +1'. Power factor for each phase. The actual values will be conveyed by one subproperty per alternating current phase: L1, L2 and L3" .

###  https://smartdatamodels.org/dataModel.Energy/displacementPowerFactor
energy:displacementPowerFactor rdf:type owl:ObjectProperty ;
                               rdfs:subPropertyOf :Property ;
                               rdfs:domain [ rdf:type owl:Class ;
                                             owl:unionOf ( energy:ACMeasurement
                                                           energy:ThreePhaseAcMeasurement
                                                         )
                                           ] ;
                               rdfs:range default:displacementPowerFactorType ;
                               rdfs:comment "Property. Model:'http://schema.org/StructuredValue'. Units:'-1 to +1'. Displacement power factor for each phase. The quantity is based on the fundamental frequency of the system. The actual values will be conveyed by one subproperty per alternating current phase: L1, L2 and L3" .

###  https://smartdatamodels.org/dataModel.Energy/current
energy:current rdf:type owl:ObjectProperty ;
               rdfs:subPropertyOf :Property ;
               rdfs:domain [ rdf:type owl:Class ;
                             owl:unionOf ( energy:ACMeasurement
                                           energy:ThreePhaseAcMeasurement
                                         )
                           ] ;
               rdfs:range default:currentType ;
               rdfs:comment "Property. Model:'http://schema.org/StructuredValue'. Units:'Ampers (A)'. Electrical current. The actual values will be conveyed by one subproperty per alternating current phase and the neutral wire: L1, L2, L3 and N" .

###  https://smartdatamodels.org/dataModel.Energy/phaseVoltage
energy:phaseVoltage rdf:type owl:ObjectProperty ;
                    rdfs:subPropertyOf :Property ;
                    rdfs:domain [ rdf:type owl:Class ;
                                  owl:unionOf ( energy:ACMeasurement
                                                energy:ThreePhaseAcMeasurement
                                              )
                                ] ;
                    rdfs:range default:phaseVoltageType ;
                    rdfs:comment "Property. Model:'http://schema.org/StructuredValue'. Units:'Volts (V)'. The voltage between each phase and neutral conductor. The actual values will be conveyed by one subproperty per alternating current phase: L1, L2 and L3" .

###  https://smartdatamodels.org/dataModel.Energy/thdVoltage
energy:thdVoltage rdf:type owl:ObjectProperty ;
                  rdfs:subPropertyOf :Property ;
                  rdfs:domain [ rdf:type owl:Class ;
                                owl:unionOf ( energy:ACMeasurement
                                              energy:ThreePhaseAcMeasurement
                                            )
                              ] ;
                  rdfs:range default:thdVoltageType ;
                  rdfs:comment "Property. Model:'http://schema.org/StructuredValue'. Units:'0 to 1'. Total harmonic distortion of voltage for each phase. The actual values will be conveyed by one subproperty per alternating current phase: L1, L2 and L3" .

###  https://smartdatamodels.org/dataModel.Energy/thdCurrent
energy:thdCurrent rdf:type owl:ObjectProperty ;
                  rdfs:subPropertyOf :Property ;
                  rdfs:domain [ rdf:type owl:Class ;
                                owl:unionOf ( energy:ACMeasurement
                                              energy:ThreePhaseAcMeasurement
                                            )
                              ] ;
                  rdfs:range default:thdCurrentType ;
                  rdfs:comment "Property. Model:'http://schema.org/StructuredValue'. Units:'0 to 1'. Total harmonic distortion of electrical current. The actual values will be conveyed by one subproperty per alternating current phase: L1, L2 and L3" .

###  https://smartdatamodels.org/dataModel.Energy/phaseToPhaseVoltage
energy:phaseToPhaseVoltage rdf:type owl:ObjectProperty ;
                           rdfs:subPropertyOf :Property ;
                           rdfs:domain [ rdf:type owl:Class ;
                                         owl:unionOf ( energy:ACMeasurement
                                                       energy:ThreePhaseAcMeasurement
                                                     )
                                       ] ;
                           rdfs:range default:phaseToPhaseVoltageType ;
                           rdfs:comment "Property. Model:'http://schema.org/StructuredValue'. Units:'Volts (V)'. Voltage between phases. A value for each phase pair: phases 1 and 2 (L12), phases 2 and 3 (L32), phases 3 and 1 (L31)" .

###  https://smartdatamodels.org/dataModel.Energy/refPointOfInterest
energy:refPointOfInterest rdf:type owl:ObjectProperty ;
                          rdfs:subPropertyOf :Relationship ;
                          rdfs:domain [ rdf:type owl:Class ;
                                        owl:unionOf ( energy:InverterDevice
                                                      energy:TechnicalCabinetDevice
                                                    )
                                      ] ;
                          rdfs:range :Entity ;
                          rdfs:comment "Relationship. Reference to a [PointOfInterest](https://github.com/smart-data-models/dataModel.PointOfInterest/blob/master/PointOfInterest/doc/spec.md) linked with the observation" .

###  https://smartdatamodels.org/dataModel.Energy/dimension
energy:dimension rdf:type owl:ObjectProperty ;
                 rdfs:subPropertyOf :Property ;
                 rdfs:domain [ rdf:type owl:Class ;
                               owl:unionOf ( energy:InverterDevice
                                             energy:TechnicalCabinetDevice
                                           )
                             ] ;
                 rdfs:range default:dimensionType ;
                 rdfs:comment "Property. The format is structured by a sub-property of 3 items. The unit code (text) of measurement  is given using the [UN/CEFACT Common Codes](http://wiki.goodrelations-vocabulary.org/Documentation/UN/CEFACT_Common_Codes). For instance, **CMT** represents Centimeter" .

###  https://smartdatamodels.org/dataModel.Energy/operatingTemperature
energy:operatingTemperature rdf:type owl:ObjectProperty ;
                            rdfs:subPropertyOf :Property ;
                            rdfs:domain [ rdf:type owl:Class ;
                                          owl:unionOf ( energy:InverterDevice
                                                        energy:TechnicalCabinetDevice
                                                      )
                                        ] ;
                            rdfs:range default:operatingTemperatureType ;
                            rdfs:comment "Property. Ambient operating temperature range. This is the minimum and maximum resistance to cold and heat. The format is structured by a sub-property of 2 items. The unit code (text) is given using the [UN/CEFACT Common Codes](http://wiki.goodrelations-vocabulary.org/Documentation/UN/CEFACT_Common_Codes). For instance, **CEL** represents Degree Celsius" .

###  https://smartdatamodels.org/dataModel.Energy/operatingAirHumidity
energy:operatingAirHumidity rdf:type owl:ObjectProperty ;
                            rdfs:subPropertyOf :Property ;
                            rdfs:domain energy:InverterDevice ;
                            rdfs:range default:operatingAirHumidityType ;
                            rdfs:comment "Property. Ambient operating Air Humidity range. The format is structured by a sub-property of 2 items. The unit code (text) is given using the [UN/CEFACT Common Codes](http://wiki.goodrelations-vocabulary.org/Documentation/UN/CEFACT_Common_Codes). For instance, **P1** represents Percent" .

###  https://smartdatamodels.org/dataModel.Energy/operatingVoltageDC
energy:operatingVoltageDC rdf:type owl:ObjectProperty ;
                          rdfs:subPropertyOf :Property ;
                          rdfs:domain energy:InverterDevice ;
                          rdfs:range default:operatingVoltageDCType ;
                          rdfs:comment "Property. Minimum and Maximum voltage allowed. The format is structured by a sub-property of 2 items. The unit code (text) is given using the [UN/CEFACT Common Codes](http://wiki.goodrelations-vocabulary.org/Documentation/UN/CEFACT_Common_Codes). For instance, **VLT** represents Volt.. Model:'https://schema.org/Number'. Units:'Volt'" .

###  https://smartdatamodels.org/dataModel.Energy/operatingAmpereDC
energy:operatingAmpereDC rdf:type owl:ObjectProperty ;
                         rdfs:subPropertyOf :Property ;
                         rdfs:domain energy:InverterDevice ;
                         rdfs:range default:operatingAmpereDCType ;
                         rdfs:comment "Property. Minimum and Maximum Ampere allowed.. The format is structured by a sub-property of 2 items. The unit code (text) is given using the [UN/CEFACT Common Codes](http://wiki.goodrelations-vocabulary.org/Documentation/UN/CEFACT_Common_Codes). For instance, **AMP** represents Ampere. Model:'https://schema.org/Number'. Units:'Ampere'" .

###  https://smartdatamodels.org/dataModel.Energy/operatingFrequencyDC
energy:operatingFrequencyDC rdf:type owl:ObjectProperty ;
                            rdfs:subPropertyOf :Property ;
                            rdfs:domain energy:InverterDevice ;
                            rdfs:range default:operatingFrequencyDCType ;
                            rdfs:comment "Property. Minimum and Maximum Frequency allowed. The format is structured by a sub-property of 2 items. The unit code (text) is given using the [UN/CEFACT Common Codes](http://wiki.goodrelations-vocabulary.org/Documentation/UN/CEFACT_Common_Codes). For instance, **HTZ** represents Hertz. Model:'https://schema.org/Number'. Units:'Hertz'" .

###  https://smartdatamodels.org/dataModel.Energy/mPPTPVVoltageDC
energy:mPPTPVVoltageDC rdf:type owl:ObjectProperty ;
                       rdfs:subPropertyOf :Property ;
                       rdfs:domain energy:InverterDevice ;
                       rdfs:range default:mPPTPVVoltageDCType ;
                       rdfs:comment "Property. Minimum and Maximum Photo-voltaic voltage range, MPPT allowed. The format is structured by a sub-property of 2 items. The unit code (text) is given using the [UN/CEFACT Common Codes](http://wiki.goodrelations-vocabulary.org/Documentation/UN/CEFACT_Common_Codes). For instance, **VLT** represents Volt. Model:'https://schema.org/Number'. Units:'Volt'" .

###  https://smartdatamodels.org/dataModel.Energy/operatingVoltageAC
energy:operatingVoltageAC rdf:type owl:ObjectProperty ;
                          rdfs:subPropertyOf :Property ;
                          rdfs:domain energy:InverterDevice ;
                          rdfs:range default:operatingVoltageACType ;
                          rdfs:comment "Property. Minimum and Maximum voltage allowed. The format is structured by a sub-property of 2 items. The unit code (text) is given using the [UN/CEFACT Common Codes](http://wiki.goodrelations-vocabulary.org/Documentation/UN/CEFACT_Common_Codes). For instance, **VLT** represents Volt. Units:'Volt'. Model:'http://schema.org/StructuredValue'" .

###  https://smartdatamodels.org/dataModel.Energy/operatingAmpereAC
energy:operatingAmpereAC rdf:type owl:ObjectProperty ;
                         rdfs:subPropertyOf :Property ;
                         rdfs:domain energy:InverterDevice ;
                         rdfs:range default:operatingAmpereACType ;
                         rdfs:comment "Property. Minimum and Maximum Ampere allowed.. The format is structured by a sub-property of 2 items. The unit code (text) is given using the [UN/CEFACT Common Codes](http://wiki.goodrelations-vocabulary.org/Documentation/UN/CEFACT_Common_Codes). For instance, **AMP** represents Ampere. Model:'http://schema.org/Number'. Units:'Ampere'" .

###  https://smartdatamodels.org/dataModel.Energy/operatingFrequencyAC
energy:operatingFrequencyAC rdf:type owl:ObjectProperty ;
                            rdfs:subPropertyOf :Property ;
                            rdfs:domain energy:InverterDevice ;
                            rdfs:range default:operatingFrequencyACType ;
                            rdfs:comment "Property. Minimum and Maximum Frequency allowed. The format is structured by a sub-property of 2 items. The unit code (text) is given using the [UN/CEFACT Common Codes](http://wiki.goodrelations-vocabulary.org/Documentation/UN/CEFACT_Common_Codes). For instance, **HTZ** represents Hertz. Units:'Volt'. Model:'http://schema.org/StructuredValue'. Units:'Hertz'" .

###  https://smartdatamodels.org/dataModel.Energy/moduleYieldRate
energy:moduleYieldRate rdf:type owl:ObjectProperty ;
                       rdfs:subPropertyOf :Property ;
                       rdfs:domain energy:InverterDevice ;
                       rdfs:range default:moduleYieldRateType ;
                       rdfs:comment "Property. Yield Rate of the Device. The format is structured by a sub-property of 2 items (European Standard - Manufacturer Standard). The unit code (text) is given using the [UN/CEFACT Common Codes](http://wiki.goodrelations-vocabulary.org/Documentation/UN/CEFACT_Common_Codes). For instance, **P1** represents Percent. Model:'http://schema.org/StructuredValue'" .

###  https://smartdatamodels.org/dataModel.Energy/refDeviceList
energy:refDeviceList rdf:type owl:ObjectProperty ;
                     rdfs:subPropertyOf :Relationship ;
                     rdfs:domain energy:TechnicalCabinetDevice ;
                     rdfs:range :Entity ;
                     rdfs:comment "Relationship. A list of reference to the [Devices](https://github.com/smart-data-models/dataModel.Device/blob/master/Device/doc/spec.md) which are inside the technical Cabinet Device" .

###  https://smartdatamodels.org/dataModel.Energy/internalDimension
energy:internalDimension rdf:type owl:ObjectProperty ;
                         rdfs:subPropertyOf :Property ;
                         rdfs:domain energy:TechnicalCabinetDevice ;
                         rdfs:range default:internalDimensionType ;
                         rdfs:comment "Property. Internal dimension corresponding to the place to work inside the technical cabinet. The format is structured by a sub-property of 3 items. The unit code (text) of measurement  is given using the [UN/CEFACT Common Codes](http://wiki.goodrelations-vocabulary.org/Documentation/UN/CEFACT_Common_Codes). For instance, **CMT** represents Centimeter. Model:'https://schema.org/StructuredValue'" .

#################################################################
#    Data Properties
#################################################################

###  https://uri.etsi.org/ngsi-ld/TemporalProperty
:TemporalProperty rdf:type owl:DatatypeProperty .

###  https://uri.etsi.org/ngsi-ld/createdAt
:createdAt rdf:type owl:DatatypeProperty ;
           rdfs:range xsd:dateTime .

###  https://uri.etsi.org/ngsi-ld/hasValue
:hasValue rdf:type owl:DatatypeProperty ;
          rdfs:domain :Property .

###  https://uri.etsi.org/ngsi-ld/hasLanguageMap
:hasLanguageMap rdf:type owl:DatatypeProperty ;
                rdfs:domain :LanguageProperty ;
                rdfs:range :LanguageMap .

###  https://uri.etsi.org/ngsi-ld/modifiedAt
:modifiedAt rdf:type owl:DatatypeProperty ;
            rdfs:range xsd:dateTime .

###  https://uri.etsi.org/ngsi-ld/observedAt
:observedAt rdf:type owl:DatatypeProperty ;
            rdfs:range xsd:dateTime .

###  https://uri.etsi.org/ngsi-ld/unitCode
:unitCode rdf:type owl:DatatypeProperty ;
          rdfs:range xsd:string .

###  https://uri.etsi.org/ngsi-ld/scope
:scope rdf:type owl:DatatypeProperty ;
       rdfs:range xsd:string .

###  https://uri.etsi.org/ngsi-ld/coordinates
:coordinates rdf:type owl:DatatypeProperty ;
             rdfs:domain :Geometry ;
             rdfs:range rdf:List .

###  https://uri.etsi.org/ngsi-ld/bbox
:bbox rdf:type owl:DatatypeProperty ;
      rdfs:domain :Geometry ;
      rdfs:range rdf:List .

###  https://smartdatamodels.org/dateCreated
smart:dateCreated rdf:type owl:DatatypeProperty ;
                  rdfs:subPropertyOf :Property ;
                  rdfs:domain [ rdf:type owl:Class ;
                                owl:unionOf ( building:BuildingOperation
                                              building:Building
                                              building:VibrationsObserved
                                              energy:ACMeasurement
                                              energy:InverterDevice
                                              energy:TechnicalCabinetDevice
                                              energy:ThreePhaseAcMeasurement
                                            )
                              ] ;
                  rdfs:range xsd:dateTime ;
                  rdfs:comment "Property. Entity creation timestamp. This will usually be allocated by the storage platform" .

###  https://smartdatamodels.org/dateModified
smart:dateModified rdf:type owl:DatatypeProperty ;
                   rdfs:subPropertyOf :Property ;
                   rdfs:domain [ rdf:type owl:Class ;
                                 owl:unionOf ( building:BuildingOperation
                                               building:Building
                                               building:VibrationsObserved
                                               energy:ACMeasurement
                                               energy:InverterDevice
                                               energy:TechnicalCabinetDevice
                                               energy:ThreePhaseAcMeasurement
                                             )
                               ] ;
                   rdfs:range xsd:dateTime ;
                   rdfs:comment "Property. Timestamp of the last modification of the entity. This will usually be allocated by the storage platform" .

###  https://smartdatamodels.org/source
smart:source rdf:type owl:DatatypeProperty ;
             rdfs:subPropertyOf :Property ;
             rdfs:domain [ rdf:type owl:Class ;
                           owl:unionOf ( building:BuildingOperation
                                         building:Building
                                         building:VibrationsObserved
                                         energy:ACMeasurement
                                         energy:InverterDevice
                                         energy:TechnicalCabinetDevice
                                         energy:ThreePhaseAcMeasurement
                                       )
                         ] ;
             rdfs:range xsd:string ;
             rdfs:comment "Property. A sequence of characters giving the original source of the entity data as a URL. Recommended to be the fully qualified domain name of the source provider, or the URL to the source object" .

###  https://smartdatamodels.org/name
smart:name rdf:type owl:DatatypeProperty ;
           rdfs:subPropertyOf :Property ;
           rdfs:domain [ rdf:type owl:Class ;
                         owl:unionOf ( building:BuildingOperation
                                       building:Building
                                       building:VibrationsObserved
                                       energy:ACMeasurement
                                       energy:InverterDevice
                                       energy:TechnicalCabinetDevice
                                       energy:ThreePhaseAcMeasurement
                                     )
                       ] ;
           rdfs:range xsd:string ;
           rdfs:comment "Property. The name of this item" .

###  https://smartdatamodels.org/alternateName
smart:alternateName rdf:type owl:DatatypeProperty ;
                    rdfs:subPropertyOf :Property ;
                    rdfs:domain [ rdf:type owl:Class ;
                                  owl:unionOf ( building:BuildingOperation
                                                building:Building
                                                building:VibrationsObserved
                                                energy:ACMeasurement
                                                energy:InverterDevice
                                                energy:TechnicalCabinetDevice
                                                energy:ThreePhaseAcMeasurement
                                              )
                                ] ;
                    rdfs:range xsd:string ;
                    rdfs:comment "Property. An alternative name for this item" .

###  http://purl.org/dc/terms/description
purlterms:description rdf:type owl:DatatypeProperty ;
                      rdfs:subPropertyOf :Property ;
                      rdfs:domain [ rdf:type owl:Class ;
                                    owl:unionOf ( building:BuildingOperation
                                                  building:Building
                                                  building:VibrationsObserved
                                                  energy:ACMeasurement
                                                  energy:InverterDevice
                                                  energy:TechnicalCabinetDevice
                                                  energy:ThreePhaseAcMeasurement
                                                )
                                  ] ;
                      rdfs:range xsd:string ;
                      rdfs:comment "Property. A description of this item" .

###  https://smartdatamodels.org/dataProvider
smart:dataProvider rdf:type owl:DatatypeProperty ;
                   rdfs:subPropertyOf :Property ;
                   rdfs:domain [ rdf:type owl:Class ;
                                 owl:unionOf ( building:BuildingOperation
                                               building:Building
                                               building:VibrationsObserved
                                               energy:ACMeasurement
                                               energy:InverterDevice
                                               energy:TechnicalCabinetDevice
                                               energy:ThreePhaseAcMeasurement
                                             )
                               ] ;
                   rdfs:range xsd:string ;
                   rdfs:comment "Property. A sequence of characters identifying the provider of the harmonised data entity" .

###  https://smartdatamodels.org/seeAlso
smart:seeAlso rdf:type owl:DatatypeProperty ;
              rdfs:subPropertyOf :Property ;
              rdfs:domain building:BuildingOperation ;
              rdfs:range [ rdf:type rdfs:Datatype ;
                           owl:unionOf ( xsd:anyURI
                                         rdf:List
                                        )
                          ] ;
              rdfs:comment "Property. list of uri pointing to additional resources about the item -- item_type:xsd:anyURI." .

###  https://smartdatamodels.org/dataModel.Building/operationType
building:operationType rdf:type owl:DatatypeProperty ;
                       rdfs:subPropertyOf :Property ;
                       rdfs:domain building:BuildingOperation ;
                       rdfs:range xsd:string ;
                       rdfs:comment "Property. Model:'https://schema.org/Text'. Type of the operation on the building" .

###  https://smartdatamodels.org/dataModel.Building/result
building:result rdf:type owl:DatatypeProperty ;
                rdfs:subPropertyOf :Property ;
                rdfs:domain building:BuildingOperation ;
                rdfs:range xsd:string ;
                rdfs:comment "Property. Result of the building operation. Model:'https://schema.org/Text'. Enum:'ok, aborted'" .

###  https://smartdatamodels.org/startDate
smart:startDate rdf:type owl:DatatypeProperty ;
                rdfs:subPropertyOf :Property ;
                rdfs:domain building:BuildingOperation ;
                rdfs:range xsd:dateTime ;
                rdfs:comment "Property. Model:'https://schema.org/DateTime'. The planned start date for the operation" .

###  https://smartdatamodels.org/endDate
smart:endDate rdf:type owl:DatatypeProperty ;
              rdfs:subPropertyOf :Property ;
              rdfs:domain building:BuildingOperation ;
              rdfs:range xsd:dateTime ;
              rdfs:comment "Property. Model:'https://schema.org/DateTime'. The planned end date for the operation" .

###  https://smartdatamodels.org/dataModel.Building/dateStarted
building:dateStarted rdf:type owl:DatatypeProperty ;
                     rdfs:subPropertyOf :Property ;
                     rdfs:domain building:BuildingOperation ;
                     rdfs:range xsd:dateTime ;
                     rdfs:comment "Property. Model:'https://schema.org/DateTime'. The actual start date for the operation" .

###  https://smartdatamodels.org/dataModel.Building/dateFinished
building:dateFinished rdf:type owl:DatatypeProperty ;
                      rdfs:subPropertyOf :Property ;
                      rdfs:domain building:BuildingOperation ;
                      rdfs:range xsd:dateTime ;
                      rdfs:comment "Property. Model:'https://schema.org/DateTime'. The actual end date for the operation" .

###  ngsi-ld:status
ngsi-ld:status rdf:type owl:DatatypeProperty ;
               rdfs:subPropertyOf :Property ;
               rdfs:domain building:BuildingOperation ;
               rdfs:range xsd:string ;
               rdfs:comment "Property. Status of the operation. Model:'https://schema.org/Text'. Enum:'cancelled, finished, ongoing, planned, scheduled' " .

###  https://smartdatamodels.org/dataModel.Building/operationSequence
building:operationSequence rdf:type owl:DatatypeProperty ;
                           rdfs:subPropertyOf :Property ;
                           rdfs:domain building:BuildingOperation ;
                           rdfs:range rdf:List ;
                           rdfs:comment "Property. Model:'https://schema.org/Text'. Id of the sequence of the operation when available -- item_type:xsd:string." .

###  https://smartdatamodels.org/streetAddress
smart:streetAddress rdf:type owl:DatatypeProperty ;
                    rdfs:domain default:addressType ;
                    rdfs:range xsd:string ;
                    rdfs:comment "Property. The street address. Model:'https://schema.org/streetAddress'" .

###  https://smartdatamodels.org/addressLocality
smart:addressLocality rdf:type owl:DatatypeProperty ;
                      rdfs:domain default:addressType ;
                      rdfs:range xsd:string ;
                      rdfs:comment "Property. The locality in which the street address is, and which is in the region. Model:'https://schema.org/addressLocality'" .

###  https://smartdatamodels.org/addressRegion
smart:addressRegion rdf:type owl:DatatypeProperty ;
                    rdfs:domain default:addressType ;
                    rdfs:range xsd:string ;
                    rdfs:comment "Property. The region in which the locality is, and which is in the country. Model:'https://schema.org/addressRegion'" .

###  https://smartdatamodels.org/addressCountry
smart:addressCountry rdf:type owl:DatatypeProperty ;
                     rdfs:domain default:addressType ;
                     rdfs:range xsd:string ;
                     rdfs:comment "Property. The country. For example, Spain. Model:'https://schema.org/addressCountry'" .

###  https://smartdatamodels.org/postalCode
smart:postalCode rdf:type owl:DatatypeProperty ;
                 rdfs:domain default:addressType ;
                 rdfs:range xsd:string ;
                 rdfs:comment "Property. The postal code. For example, 24004. Model:'https://schema.org/https://schema.org/postalCode'" .

###  https://smartdatamodels.org/postOfficeBoxNumber
smart:postOfficeBoxNumber rdf:type owl:DatatypeProperty ;
                          rdfs:domain default:addressType ;
                          rdfs:range xsd:string ;
                          rdfs:comment "Property. The post office box number for PO box addresses. For example, 03578. Model:'https://schema.org/postOfficeBoxNumber'" .

###  https://smartdatamodels.org/streetNr
smart:streetNr rdf:type owl:DatatypeProperty ;
               rdfs:domain default:addressType ;
               rdfs:range xsd:string ;
               rdfs:comment "Property. Number identifying a specific property on a public street" .

###  https://smartdatamodels.org/district
smart:district rdf:type owl:DatatypeProperty ;
               rdfs:domain default:addressType ;
               rdfs:range xsd:string ;
               rdfs:comment "Property. A district is a type of administrative division that, in some countries, is managed by the local government" .

###  https://smartdatamodels.org/areaServed
smart:areaServed rdf:type owl:DatatypeProperty ;
                 rdfs:subPropertyOf :Property ;
                 rdfs:domain [ rdf:type owl:Class ;
                               owl:unionOf ( building:Building
                                             building:VibrationsObserved
                                             energy:ACMeasurement
                                             energy:InverterDevice
                                             energy:TechnicalCabinetDevice
                                             energy:ThreePhaseAcMeasurement
                                           )
                             ] ;
                 rdfs:range xsd:string ;
                 rdfs:comment "Property. The geographic area where a service or offered item is provided. Model:'https://schema.org/Text'" .

###  https://smartdatamodels.org/dataModel.Building/category
building:category rdf:type owl:DatatypeProperty ;
                  rdfs:subPropertyOf :Property ;
                  rdfs:domain building:Building ;
                  rdfs:range rdf:List ;
                  rdfs:comment "Property. Category of the building. Enum:'apartments, bakehouse, barn, bridge, bungalow, bunker, cathedral, cabin, carport, chapel, church, civic, commercial, conservatory, construction, cowshed, detached, digester, dormitory, farm, farm_auxiliary, garage, garages, garbage_shed, grandstand, greenhouse, hangar, hospital, hotel, house, houseboat, hut, industrial, kindergarten, kiosk, mosque, office, parking, pavilion, public, residential, retail, riding_hall, roof, ruins, school, service, shed, shrine, stable, stadium, static_caravan, sty, synagogue, temple, terrace, train_station, transformer_tower, transportation, university, warehouse, water_tower' -- item_type:xsd:string, item_enum:['apartments', 'bakehouse', 'barn', 'bridge', 'bungalow', 'bunker', 'cathedral', 'cabin', 'carport', 'cemetery', 'chapel', 'church', 'civic', 'commercial', 'conservatory', 'construction', 'cowshed', 'detached', 'digester', 'dormitory', 'farm', 'farm_auxiliary', 'garage', 'garages', 'garbage_shed', 'grandstand', 'greenhouse', 'hangar', 'hospital', 'hotel', 'house', 'houseboat', 'hut', 'industrial', 'kindergarten', 'kiosk', 'mosque', 'office', 'parking', 'pavilion', 'public', 'residential', 'retail', 'riding_hall', 'roof', 'ruins', 'school', 'service', 'shed', 'shrine', 'stable', 'stadium', 'static_caravan', 'sty', 'synagogue', 'temple', 'terrace', 'train_station', 'transformer_tower', 'transportation', 'university', 'warehouse', 'water_tower']." .

###  https://smartdatamodels.org/dataModel.Building/containedInPlace
building:containedInPlace rdf:type owl:DatatypeProperty ;
                          rdfs:subPropertyOf :Property ;
                          rdfs:domain building:Building ;
                          rdfs:range common:location .

###  https://smartdatamodels.org/dataModel.Building/floorsAboveGround
building:floorsAboveGround rdf:type owl:DatatypeProperty ;
                           rdfs:subPropertyOf :Property ;
                           rdfs:domain building:Building ;
                           rdfs:range xsd:integer ;
                           rdfs:comment "Property. Floors above the ground level. Model:'https://schema.org/Number'" .

###  https://smartdatamodels.org/dataModel.Building/floorsBelowGround
building:floorsBelowGround rdf:type owl:DatatypeProperty ;
                           rdfs:subPropertyOf :Property ;
                           rdfs:domain building:Building ;
                           rdfs:range xsd:integer ;
                           rdfs:comment "Property. Floors below the ground level. Model:'https://schema.org/Number'" .

###  https://smartdatamodels.org/openingHours
smart:openingHours rdf:type owl:DatatypeProperty ;
                   rdfs:subPropertyOf :Property ;
                   rdfs:domain building:Building ;
                   rdfs:range rdf:List ;
                   rdfs:comment "Property. Model:'https://schema.org/openingHours'. Opening hours of this building -- item_type:xsd:string." .

###  https://smartdatamodels.org/dataModel.Building/collapseRisk
building:collapseRisk rdf:type owl:DatatypeProperty ;
                      rdfs:subPropertyOf :Property ;
                      rdfs:domain building:Building ;
                      rdfs:range xsd:float ;
                      rdfs:comment "Property. Model:'https://schema.org/Number'. Probability of total collapse of the building" .

###  https://smartdatamodels.org/dataModel.Building/peopleCapacity
building:peopleCapacity rdf:type owl:DatatypeProperty ;
                        rdfs:subPropertyOf :Property ;
                        rdfs:domain building:Building ;
                        rdfs:range xsd:float ;
                        rdfs:comment "Property. Model:'https://schema.org/Number'. Allowed people present at the building" .

###  https://smartdatamodels.org/dataModel.Building/peopleOccupancy
building:peopleOccupancy rdf:type owl:DatatypeProperty ;
                         rdfs:subPropertyOf :Property ;
                         rdfs:domain building:Building ;
                         rdfs:range xsd:float ;
                         rdfs:comment "Property. Model:'https://schema.org/Number'. People present at the building" .

###  https://smartdatamodels.org/dateObserved
smart:dateObserved rdf:type owl:DatatypeProperty ;
                   rdfs:subPropertyOf :Property ;
                   rdfs:domain [ rdf:type owl:Class ;
                                 owl:unionOf ( building:VibrationsObserved
                                               energy:ACMeasurement
                                             )
                               ] ;
                   rdfs:range xsd:dateTime ;
                   rdfs:comment "Property. Model:'https://schema.org/DateTime'. Date and time of this observation represented by an ISO8601 UTC format. It can be represented by an specific time instant or by an ISO8601 interval to separate attributes `dateObservedFrom`,`dateObservedTo`" .

###  https://smartdatamodels.org/dataModel.Building/accelerationMeasured
building:accelerationMeasured rdf:type owl:DatatypeProperty ;
                              rdfs:subPropertyOf :Property ;
                              rdfs:domain building:VibrationsObserved ;
                              rdfs:range xsd:float ;
                              rdfs:comment "Property. Model:'https://schema.org/Number'. Magnitude of the vibrations observed (e.g. Earthquake) or other floor movements. Units:'m/s2'" .

###  https://smartdatamodels.org/dataModel.Energy/dateObservedFrom
energy:dateObservedFrom rdf:type owl:DatatypeProperty ;
                        rdfs:subPropertyOf :Property ;
                        rdfs:domain energy:ACMeasurement ;
                        rdfs:range xsd:dateTime ;
                        rdfs:comment "Property. Model:'https://schema.org/DateTime'. Observation period: Start date and time in an ISO8601 UTC format. The attribute can be used in addition to the `dateObserved` attribute when it corresponds to a time interval to be highlighted" .

###  https://smartdatamodels.org/dataModel.Energy/dateObservedTo
energy:dateObservedTo rdf:type owl:DatatypeProperty ;
                      rdfs:subPropertyOf :Property ;
                      rdfs:domain energy:ACMeasurement ;
                      rdfs:range xsd:dateTime ;
                      rdfs:comment "Property. Model:'https://schema.org/DateTime'. Observation period: End date and time in an ISO8601 UTC format. The attribute can be used in addition to the `dateObserved` attribute when it corresponds to a time interval to be highlighted" .

###  https://smartdatamodels.org/dataModel.Energy/phaseType
energy:phaseType rdf:type owl:DatatypeProperty ;
                 rdfs:subPropertyOf :Property ;
                 rdfs:domain [ rdf:type owl:Class ;
                               owl:unionOf ( energy:ACMeasurement
                                             energy:InverterDevice
                                           )
                             ] ;
                 rdfs:range xsd:string ;
                 rdfs:comment "Property. Type of Phase. A unique value. Enum:'singlePhase,threePhase'" .

###  https://smartdatamodels.org/dataModel.Energy/frequency
energy:frequency rdf:type owl:DatatypeProperty ;
                 rdfs:subPropertyOf :Property ;
                 rdfs:domain [ rdf:type owl:Class ;
                               owl:unionOf ( energy:ACMeasurement
                                             energy:ThreePhaseAcMeasurement
                                           )
                             ] ;
                 rdfs:range xsd:float ;
                 rdfs:comment "Property. Model:'http://schema.org/Number'. Units:'Hertz (Hz)'. The frequency of the circuit" .

###  https://smartdatamodels.org/dataModel.Energy/dateEnergyMeteringStarted
energy:dateEnergyMeteringStarted rdf:type owl:DatatypeProperty ;
                                 rdfs:subPropertyOf :Property ;
                                 rdfs:domain [ rdf:type owl:Class ;
                                               owl:unionOf ( energy:ACMeasurement
                                                             energy:ThreePhaseAcMeasurement
                                                           )
                                             ] ;
                                 rdfs:range xsd:dateTime ;
                                 rdfs:comment "Property. Model:'http://schema.org/DateTime'. The starting date for metering energy" .

###  https://smartdatamodels.org/dataModel.Energy/L1
energy:L1 rdf:type owl:DatatypeProperty ;
          rdfs:domain [ rdf:type owl:Class ;
                        owl:unionOf ( default:activeEnergyImportType
                                      default:reactiveEnergyImportType
                                      default:apparentEnergyImportType
                                      default:activeEnergyExportType
                                      default:reactiveEnergyExportType
                                      default:apparentEnergyExportType
                                      default:activePowerType
                                      default:reactivePowerType
                                      default:apparentPowerType
                                      default:powerFactorType
                                      default:displacementPowerFactorType
                                      default:currentType
                                      default:phaseVoltageType
                                      default:thdVoltageType
                                      default:thdCurrentType
                                    )
                      ] ;
          rdfs:range xsd:float ;
          rdfs:comment "Property. Value for phase 1 of the thd current" .

###  https://smartdatamodels.org/dataModel.Energy/L2
energy:L2 rdf:type owl:DatatypeProperty ;
          rdfs:domain [ rdf:type owl:Class ;
                        owl:unionOf ( default:activeEnergyImportType
                                      default:reactiveEnergyImportType
                                      default:apparentEnergyImportType
                                      default:activeEnergyExportType
                                      default:reactiveEnergyExportType
                                      default:apparentEnergyExportType
                                      default:activePowerType
                                      default:reactivePowerType
                                      default:apparentPowerType
                                      default:powerFactorType
                                      default:displacementPowerFactorType
                                      default:currentType
                                      default:phaseVoltageType
                                      default:thdVoltageType
                                      default:thdCurrentType
                                    )
                      ] ;
          rdfs:range xsd:float ;
          rdfs:comment "Property. Value for phase 2 of the thd current" .

###  https://smartdatamodels.org/dataModel.Energy/L3
energy:L3 rdf:type owl:DatatypeProperty ;
          rdfs:domain [ rdf:type owl:Class ;
                        owl:unionOf ( default:activeEnergyImportType
                                      default:reactiveEnergyImportType
                                      default:apparentEnergyImportType
                                      default:activeEnergyExportType
                                      default:reactiveEnergyExportType
                                      default:apparentEnergyExportType
                                      default:activePowerType
                                      default:reactivePowerType
                                      default:apparentPowerType
                                      default:powerFactorType
                                      default:displacementPowerFactorType
                                      default:currentType
                                      default:phaseVoltageType
                                      default:thdVoltageType
                                      default:thdCurrentType
                                    )
                      ] ;
          rdfs:range xsd:float ;
          rdfs:comment "Property. Value for phase 3 of the thd current" .

###  https://smartdatamodels.org/dataModel.Energy/totalActiveEnergyImport
energy:totalActiveEnergyImport rdf:type owl:DatatypeProperty ;
                               rdfs:subPropertyOf :Property ;
                               rdfs:domain [ rdf:type owl:Class ;
                                             owl:unionOf ( energy:ACMeasurement
                                                           energy:ThreePhaseAcMeasurement
                                                         )
                                           ] ;
                               rdfs:range xsd:float ;
                               rdfs:comment "Property. Model:'https://schema.org/Number'. Units:'kilowatt hour (kWh)'. Total energy imported i.e. consumed since metering started (since `dateEnergyMeteringStarted`)" .

###  https://smartdatamodels.org/dataModel.Energy/totalReactiveEnergyImport
energy:totalReactiveEnergyImport rdf:type owl:DatatypeProperty ;
                                 rdfs:subPropertyOf :Property ;
                                 rdfs:domain [ rdf:type owl:Class ;
                                               owl:unionOf ( energy:ACMeasurement
                                                             energy:ThreePhaseAcMeasurement
                                                           )
                                             ] ;
                                 rdfs:range xsd:float ;
                                 rdfs:comment "Property. Model:'https://schema.org/Number'. Units:'kilovolt-ampere-reactive-hour (kVArh)'. Total energy imported i.e. consumed (with regards to fundamental frequency reactive power) since the metering start date (`dateEnergyMeteringStarted`)" .

###  https://smartdatamodels.org/dataModel.Energy/totalApparentEnergyImport
energy:totalApparentEnergyImport rdf:type owl:DatatypeProperty ;
                                 rdfs:subPropertyOf :Property ;
                                 rdfs:domain [ rdf:type owl:Class ;
                                               owl:unionOf ( energy:ACMeasurement
                                                             energy:ThreePhaseAcMeasurement
                                                           )
                                             ] ;
                                 rdfs:range xsd:float ;
                                 rdfs:comment "Property. Model:'https://schema.org/Number'. Units:'kilovolt-ampere-hour (kVAh)'. Total energy imported i.e. consumed (with regards to apparent power) since the metering start date (`dateEnergyMeteringStarted`)" .

###  https://smartdatamodels.org/dataModel.Energy/totalActiveEnergyExport
energy:totalActiveEnergyExport rdf:type owl:DatatypeProperty ;
                               rdfs:subPropertyOf :Property ;
                               rdfs:domain [ rdf:type owl:Class ;
                                             owl:unionOf ( energy:ACMeasurement
                                                           energy:ThreePhaseAcMeasurement
                                                         )
                                           ] ;
                               rdfs:range xsd:float ;
                               rdfs:comment "Property. Model:'https://schema.org/Number'. Units:'kilowatt hour (kWh)'. Total energy exported since metering started (since `dateEnergyMeteringStarted`)" .

###  https://smartdatamodels.org/dataModel.Energy/totalReactiveEnergyExport
energy:totalReactiveEnergyExport rdf:type owl:DatatypeProperty ;
                                 rdfs:subPropertyOf :Property ;
                                 rdfs:domain [ rdf:type owl:Class ;
                                               owl:unionOf ( energy:ACMeasurement
                                                             energy:ThreePhaseAcMeasurement
                                                           )
                                             ] ;
                                 rdfs:range xsd:float ;
                                 rdfs:comment "Property. Model:'https://schema.org/Number'. Units:'kilovolt-ampere-reactive-hour (kVArh)'. Total fundamental frequency reactive energy exported since metering started (since `dateEnergyMeteringStarted`)" .

###  https://smartdatamodels.org/dataModel.Energy/totalApparentEnergyExport
energy:totalApparentEnergyExport rdf:type owl:DatatypeProperty ;
                                 rdfs:subPropertyOf :Property ;
                                 rdfs:domain [ rdf:type owl:Class ;
                                               owl:unionOf ( energy:ACMeasurement
                                                             energy:ThreePhaseAcMeasurement
                                                           )
                                             ] ;
                                 rdfs:range xsd:float ;
                                 rdfs:comment "Property. Model:'https://schema.org/Number'. Units:'kilovolt-ampere-reactive-hour (kVArh)'. Total energy exported (with regards to apparent power) since the metering start date (`dateEnergyMeteringStarted`)" .

###  https://smartdatamodels.org/dataModel.Energy/totalActivePower
energy:totalActivePower rdf:type owl:DatatypeProperty ;
                        rdfs:subPropertyOf :Property ;
                        rdfs:domain [ rdf:type owl:Class ;
                                      owl:unionOf ( energy:ACMeasurement
                                                    energy:ThreePhaseAcMeasurement
                                                  )
                                    ] ;
                        rdfs:range xsd:float ;
                        rdfs:comment "Property. Model:'http://schema.org/Number'. Units:'watt (W)'. Active power consumed (counting all phases)" .

###  https://smartdatamodels.org/dataModel.Energy/totalReactivePower
energy:totalReactivePower rdf:type owl:DatatypeProperty ;
                          rdfs:subPropertyOf :Property ;
                          rdfs:domain [ rdf:type owl:Class ;
                                        owl:unionOf ( energy:ACMeasurement
                                                      energy:ThreePhaseAcMeasurement
                                                    )
                                      ] ;
                          rdfs:range xsd:float ;
                          rdfs:comment "Property. Model:'http://schema.org/Number'. Units:'volt-ampere-reactive (VAr)'. Reactive power consumed (counting all phases)" .

###  https://smartdatamodels.org/dataModel.Energy/totalApparentPower
energy:totalApparentPower rdf:type owl:DatatypeProperty ;
                          rdfs:subPropertyOf :Property ;
                          rdfs:domain [ rdf:type owl:Class ;
                                        owl:unionOf ( energy:ACMeasurement
                                                      energy:ThreePhaseAcMeasurement
                                                    )
                                      ] ;
                          rdfs:range xsd:float ;
                          rdfs:comment "Property. Model:'http://schema.org/Number'. Units:'volt-ampere (VA)'. Apparent power consumed (counting all phases)" .

###  https://smartdatamodels.org/dataModel.Energy/totalPowerFactor
energy:totalPowerFactor rdf:type owl:DatatypeProperty ;
                        rdfs:subPropertyOf :Property ;
                        rdfs:domain [ rdf:type owl:Class ;
                                      owl:unionOf ( energy:ACMeasurement
                                                    energy:ThreePhaseAcMeasurement
                                                  )
                                    ] ;
                        rdfs:range xsd:float ;
                        rdfs:comment "Property. Model:'http://schema.org/Number'. Units:'-1 to +1'. Power factor including all phases" .

###  https://smartdatamodels.org/dataModel.Energy/totalDisplacementPowerFactor
energy:totalDisplacementPowerFactor rdf:type owl:DatatypeProperty ;
                                    rdfs:subPropertyOf :Property ;
                                    rdfs:domain [ rdf:type owl:Class ;
                                                  owl:unionOf ( energy:ACMeasurement
                                                                energy:ThreePhaseAcMeasurement
                                                              )
                                                ] ;
                                    rdfs:range xsd:float ;
                                    rdfs:comment "Property. Model:'http://schema.org/Number'. Units:'-1 to +1'. Displacement power factor including all phases. The quantity is based on the fundamental frequency of the system" .

###  https://smartdatamodels.org/dataModel.Energy/N
energy:N rdf:type owl:DatatypeProperty ;
         rdfs:domain default:currentType ;
         rdfs:range xsd:float ;
         rdfs:comment "Property. Value for phase neutral of the current" .

###  https://smartdatamodels.org/dataModel.Energy/L12
energy:L12 rdf:type owl:DatatypeProperty ;
           rdfs:domain default:phaseToPhaseVoltageType ;
           rdfs:range xsd:float ;
           rdfs:comment "Property. Value for phase 1 to phase 2 voltage" .

###  https://smartdatamodels.org/dataModel.Energy/L23
energy:L23 rdf:type owl:DatatypeProperty ;
           rdfs:domain default:phaseToPhaseVoltageType ;
           rdfs:range xsd:float ;
           rdfs:comment "Property. Value for phase 2 to phase 3 voltage" .

###  https://smartdatamodels.org/dataModel.Energy/L31
energy:L31 rdf:type owl:DatatypeProperty ;
           rdfs:domain default:phaseToPhaseVoltageType ;
           rdfs:range xsd:float ;
           rdfs:comment "Property. Value for phase 3 to phase 1 voltage" .

###  https://smartdatamodels.org/dataModel.Energy/dateLastReported
energy:dateLastReported rdf:type owl:DatatypeProperty ;
                        rdfs:subPropertyOf :Property ;
                        rdfs:domain [ rdf:type owl:Class ;
                                      owl:unionOf ( energy:InverterDevice
                                                    energy:TechnicalCabinetDevice
                                                  )
                                    ] ;
                        rdfs:range xsd:dateTime ;
                        rdfs:comment "Property. A timestamp which denotes the last time when the device successfully reported data. Date and time in an ISO8601 UTCformat. Model:'https://schema.org/DateTime'" .

###  https://smartdatamodels.org/dataModel.Energy/brandName
energy:brandName rdf:type owl:DatatypeProperty ;
                 rdfs:subPropertyOf :Property ;
                 rdfs:domain [ rdf:type owl:Class ;
                               owl:unionOf ( energy:InverterDevice
                                             energy:TechnicalCabinetDevice
                                           )
                             ] ;
                 rdfs:range xsd:string ;
                 rdfs:comment "Property. Name of the brand. Model:'https://schema.org/brand'" .

###  https://smartdatamodels.org/dataModel.Energy/modelName
energy:modelName rdf:type owl:DatatypeProperty ;
                 rdfs:subPropertyOf :Property ;
                 rdfs:domain [ rdf:type owl:Class ;
                               owl:unionOf ( energy:InverterDevice
                                             energy:TechnicalCabinetDevice
                                           )
                             ] ;
                 rdfs:range xsd:string ;
                 rdfs:comment "Property. Name of the model as given by the manufacturer" .

###  https://smartdatamodels.org/dataModel.Energy/manufacturerName
energy:manufacturerName rdf:type owl:DatatypeProperty ;
                        rdfs:subPropertyOf :Property ;
                        rdfs:domain [ rdf:type owl:Class ;
                                      owl:unionOf ( energy:InverterDevice
                                                    energy:TechnicalCabinetDevice
                                                  )
                                    ] ;
                        rdfs:range xsd:string ;
                        rdfs:comment "Property. Name of the manufacturer. Model:'https://schema.org/manufacturer'" .

###  https://smartdatamodels.org/dataModel.Energy/serialNumber
energy:serialNumber rdf:type owl:DatatypeProperty ;
                    rdfs:subPropertyOf :Property ;
                    rdfs:domain [ rdf:type owl:Class ;
                                  owl:unionOf ( energy:InverterDevice
                                                energy:TechnicalCabinetDevice
                                              )
                                ] ;
                    rdfs:range xsd:string ;
                    rdfs:comment "Property. Serial number of the container. Model:'https://schema.org/serialNumber'" .

###  https://smartdatamodels.org/dataModel.Energy/application
energy:application rdf:type owl:DatatypeProperty ;
                   rdfs:subPropertyOf :Property ;
                   rdfs:domain [ rdf:type owl:Class ;
                                 owl:unionOf ( energy:InverterDevice
                                               energy:TechnicalCabinetDevice
                                             )
                               ] ;
                   rdfs:range rdf:List ;
                   rdfs:comment "Property. Target application of the Device regarding the environment. A combination of these values. Enum:'commercial, distributionService, industrial, other, publicWorks, road, tertiary, urbanService' -- item_type:xsd:string, item_enum:['commercial', 'distributionService', 'industrial', 'other', 'publicWorks', 'road', 'tertiary', 'urbanService']." .

###  https://smartdatamodels.org/dataModel.Energy/typeOfUse
energy:typeOfUse rdf:type owl:DatatypeProperty ;
                 rdfs:subPropertyOf :Property ;
                 rdfs:domain [ rdf:type owl:Class ;
                               owl:unionOf ( energy:InverterDevice
                                             energy:TechnicalCabinetDevice
                                           )
                             ] ;
                 rdfs:range xsd:string ;
                 rdfs:comment "Property. Accepted use regarding its positioning in an indoor / outdoor environment. A unique value of these values. Enum:'indoor, mixed, outdoor, other'" .

###  https://smartdatamodels.org/dataModel.Energy/installationMode
energy:installationMode rdf:type owl:DatatypeProperty ;
                        rdfs:subPropertyOf :Property ;
                        rdfs:domain [ rdf:type owl:Class ;
                                      owl:unionOf ( energy:InverterDevice
                                                    energy:TechnicalCabinetDevice
                                                  )
                                    ] ;
                        rdfs:range xsd:string ;
                        rdfs:comment "Property. Positioning of the device in relation to a ground reference system. Model:'https://schema.org/Text'. Enum:'aerial, ground, other, pole, roofing, underground, wall'" .

###  https://smartdatamodels.org/dataModel.Energy/installationCondition
energy:installationCondition rdf:type owl:DatatypeProperty ;
                             rdfs:subPropertyOf :Property ;
                             rdfs:domain [ rdf:type owl:Class ;
                                           owl:unionOf ( energy:InverterDevice
                                                         energy:TechnicalCabinetDevice
                                                       )
                                         ] ;
                             rdfs:range rdf:List ;
                             rdfs:comment "Property. Condition and possibility of use in the following environments. A combination of these values. Enum:'desert, dust, extremeCold, extremeClimate, extremeHeat, extremeHumidity, marine, none, other, saline, seismic, sand' -- item_type:xsd:string, item_enum:['desert', 'dust', 'extremeCold', 'extremeClimate', 'extremeHeat', 'extremeHumidity', 'marine', 'none', 'other', 'saline', 'seismic', 'sand']." .

###  https://smartdatamodels.org/dataModel.Energy/possibilityOfUse
energy:possibilityOfUse rdf:type owl:DatatypeProperty ;
                        rdfs:subPropertyOf :Property ;
                        rdfs:domain [ rdf:type owl:Class ;
                                      owl:unionOf ( energy:InverterDevice
                                                    energy:TechnicalCabinetDevice
                                                  )
                                    ] ;
                        rdfs:range xsd:string ;
                        rdfs:comment "Property. Possibility of use. A unique value. Enum:'mixed, mobile, other, stationary'" .

###  https://smartdatamodels.org/dataModel.Energy/documentation
energy:documentation rdf:type owl:DatatypeProperty ;
                     rdfs:subPropertyOf :Property ;
                     rdfs:domain [ rdf:type owl:Class ;
                                   owl:unionOf ( energy:InverterDevice
                                                 energy:TechnicalCabinetDevice
                                               )
                                 ] ;
                     rdfs:range xsd:string ;
                     rdfs:comment "Property. A link to device's documentation. Model:'https://schema.org/URL'" .

###  https://smartdatamodels.org/dataModel.Energy/supplyPhaseNb
energy:supplyPhaseNb rdf:type owl:DatatypeProperty ;
                     rdfs:subPropertyOf :Property ;
                     rdfs:domain energy:InverterDevice ;
                     rdfs:range xsd:float ;
                     rdfs:comment "Property. Number of power supply phases. Model:'https://schema.org/Number'" .

###  https://smartdatamodels.org/dataModel.Energy/length
energy:length rdf:type owl:DatatypeProperty ;
              rdfs:domain default:dimensionType ;
              rdfs:range xsd:float .

###  https://smartdatamodels.org/dataModel.Energy/height
energy:height rdf:type owl:DatatypeProperty ;
              rdfs:domain [ rdf:type owl:Class ;
                            owl:unionOf ( default:dimensionType
                                          default:internalDimensionType
                                        )
                          ] ;
              rdfs:range xsd:float .

###  https://smartdatamodels.org/dataModel.Energy/depth
energy:depth rdf:type owl:DatatypeProperty ;
             rdfs:domain [ rdf:type owl:Class ;
                           owl:unionOf ( default:dimensionType
                                         default:internalDimensionType
                                       )
                         ] ;
             rdfs:range xsd:float .

###  https://smartdatamodels.org/dataModel.Energy/weight
energy:weight rdf:type owl:DatatypeProperty ;
              rdfs:subPropertyOf :Property ;
              rdfs:domain [ rdf:type owl:Class ;
                            owl:unionOf ( energy:InverterDevice
                                          energy:TechnicalCabinetDevice
                                        )
                          ] ;
              rdfs:range xsd:float ;
              rdfs:comment "Property. Weight of the item. The unit code (text) of measurement  is given using the [UN/CEFACT Common Codes](http://wiki.goodrelations-vocabulary.org/Documentation/UN/CEFACT_Common_Codes). For instance, **KGM** represents Kilograms. Model:'https://schema.org/weigth'" .

###  https://smartdatamodels.org/dataModel.Energy/protectionIP
energy:protectionIP rdf:type owl:DatatypeProperty ;
                    rdfs:subPropertyOf :Property ;
                    rdfs:domain [ rdf:type owl:Class ;
                                  owl:unionOf ( energy:InverterDevice
                                                energy:TechnicalCabinetDevice
                                              )
                                ] ;
                    rdfs:range xsd:string ;
                    rdfs:comment "Property. IP 'Ingress Protection' for the Junction Box. This is the level classifies and rates the degree of protection provided by mechanical casings and electrical enclosures against intrusion, dust, accidental contact, and water according to International Electrotechnical Commission standard (EN 60-529). First digit: Solid particle protection (Single numeral: 06 or 'X'). Second digit: Liquid ingress protection (Single numeral: 09 or 'X' ).Third digit: Personal Protection against access to dangerous parts (optional additional letter). Fourth digit: Other protections (optional additional letter)" .

###  https://smartdatamodels.org/dataModel.Energy/protectionIK
energy:protectionIK rdf:type owl:DatatypeProperty ;
                    rdfs:subPropertyOf :Property ;
                    rdfs:domain [ rdf:type owl:Class ;
                                  owl:unionOf ( energy:InverterDevice
                                                energy:TechnicalCabinetDevice
                                              )
                                ] ;
                    rdfs:range xsd:float ;
                    rdfs:comment "Property. IK '*Mecanic Protection*' level relating to numeric classification for the degrees of protection provided by enclosures for electrical equipment against external mechanical impacts, according to International Electro technical Commission standard (EN 62-262). - IK varies from 0 (minimum resistance) to 10 (maximum resistance) which represents an Impact Energy (Unit Joule)" .

###  https://smartdatamodels.org/dataModel.Energy/protectionClassSLK
energy:protectionClassSLK rdf:type owl:DatatypeProperty ;
                          rdfs:subPropertyOf :Property ;
                          rdfs:domain energy:InverterDevice ;
                          rdfs:range xsd:string ;
                          rdfs:comment "Property. Protection class (SKL). - 0 : main insulation without earth connection. - 1 : main insulation and additional insulation (earth terminal). - 2 : double or reinforced insulation (equivalent to twice the main insulation) without accessible metal part. - 3 : operating in very low safety voltage (SELV) (50V maximum)" .

###  https://smartdatamodels.org/dataModel.Energy/overVoltageCategory
energy:overVoltageCategory rdf:type owl:DatatypeProperty ;
                           rdfs:subPropertyOf :Property ;
                           rdfs:domain energy:InverterDevice ;
                           rdfs:range xsd:string ;
                           rdfs:comment "Property. Over voltage category. - I : connection to circuits with transient over voltages at an appropriate low level. - II : main insulation and additional insulation (earth terminal). - III : fixed installations with reliability and availability making subject to specific specifications. - IV : materials at the origin of the electrical installation such as electric meters and main materials over current protection" .

###  ngsi-ld:min
ngsi-ld:min rdf:type owl:DatatypeProperty ;
            rdfs:domain [ rdf:type owl:Class ;
                          owl:unionOf ( default:operatingTemperatureType
                                        default:operatingAirHumidityType
                                        default:operatingVoltageDCType
                                        default:operatingAmpereDCType
                                        default:operatingFrequencyDCType
                                        default:mPPTPVVoltageDCType
                                        default:operatingVoltageACType
                                        default:operatingAmpereACType
                                        default:operatingFrequencyACType
                                      )
                        ] ;
            rdfs:range xsd:float .

###  ngsi-ld:max
ngsi-ld:max rdf:type owl:DatatypeProperty ;
            rdfs:domain [ rdf:type owl:Class ;
                          owl:unionOf ( default:operatingTemperatureType
                                        default:operatingAirHumidityType
                                        default:operatingVoltageDCType
                                        default:operatingAmpereDCType
                                        default:operatingFrequencyDCType
                                        default:mPPTPVVoltageDCType
                                        default:operatingVoltageACType
                                        default:operatingAmpereACType
                                        default:operatingFrequencyACType
                                      )
                        ] ;
            rdfs:range xsd:float .

###  https://smartdatamodels.org/dataModel.Energy/nominalPowerDC
energy:nominalPowerDC rdf:type owl:DatatypeProperty ;
                      rdfs:subPropertyOf :Property ;
                      rdfs:domain energy:InverterDevice ;
                      rdfs:range xsd:float ;
                      rdfs:comment "Property. Nominal Power or Maximum Power factor for cos phi=1. The unit code (text) is given using the [UN/CEFACT Common Codes](http://wiki.goodrelations-vocabulary.org/Documentation/UN/CEFACT_Common_Codes). For instance, **WTT** represents Watt. Model:'https://schema.org/Number'. Units:'Watt'" .

###  https://smartdatamodels.org/dataModel.Energy/nominalVoltageDC
energy:nominalVoltageDC rdf:type owl:DatatypeProperty ;
                        rdfs:subPropertyOf :Property ;
                        rdfs:domain energy:InverterDevice ;
                        rdfs:range xsd:float ;
                        rdfs:comment "Property. Nominal voltage. The unit code (text) is given using the [UN/CEFACT Common Codes](http://wiki.goodrelations-vocabulary.org/Documentation/UN/CEFACT_Common_Codes). For instance, **VLT** represents Volt. Model:'https://schema.org/Number'. Units:'Volt'" .

###  https://smartdatamodels.org/dataModel.Energy/nominalAmpereDC
energy:nominalAmpereDC rdf:type owl:DatatypeProperty ;
                       rdfs:subPropertyOf :Property ;
                       rdfs:domain energy:InverterDevice ;
                       rdfs:range xsd:float ;
                       rdfs:comment "Property. Nominal Amperage. The unit code (text) is given using the [UN/CEFACT Common Codes](http://wiki.goodrelations-vocabulary.org/Documentation/UN/CEFACT_Common_Codes). For instance, **AMP** represents Ampere. Model:'https://schema.org/Number'. Units:'Ampere'" .

###  https://smartdatamodels.org/dataModel.Energy/nominalFrequencyDC
energy:nominalFrequencyDC rdf:type owl:DatatypeProperty ;
                          rdfs:subPropertyOf :Property ;
                          rdfs:domain energy:InverterDevice ;
                          rdfs:range xsd:float ;
                          rdfs:comment "Property.  Nominal Frequency. The unit code (text) is given using the [UN/CEFACT Common Codes](http://wiki.goodrelations-vocabulary.org/Documentation/UN/CEFACT_Common_Codes). For instance, **HTZ** represents Hertz. Model:'https://schema.org/Number'. Units:'Hertz'" .

###  https://smartdatamodels.org/dataModel.Energy/startingVoltageDC
energy:startingVoltageDC rdf:type owl:DatatypeProperty ;
                         rdfs:subPropertyOf :Property ;
                         rdfs:domain energy:InverterDevice ;
                         rdfs:range xsd:float ;
                         rdfs:comment "Property. Starting voltage. The unit code (text) is given using the [UN/CEFACT Common Codes](http://wiki.goodrelations-vocabulary.org/Documentation/UN/CEFACT_Common_Codes). For instance, **VLT** represents Volt. Model:'https://schema.org/Number'. Units:'Volt'" .

###  https://smartdatamodels.org/dataModel.Energy/nbMPPTrackersDC
energy:nbMPPTrackersDC rdf:type owl:DatatypeProperty ;
                       rdfs:subPropertyOf :Property ;
                       rdfs:domain energy:InverterDevice ;
                       rdfs:range xsd:float ;
                       rdfs:comment "Property. Number of MPP trackers. Model:'https://schema.org/Number'" .

###  https://smartdatamodels.org/dataModel.Energy/nbInputParallelDC
energy:nbInputParallelDC rdf:type owl:DatatypeProperty ;
                         rdfs:subPropertyOf :Property ;
                         rdfs:domain energy:InverterDevice ;
                         rdfs:range xsd:string ;
                         rdfs:comment "Property. Maximum Number of inputs (in parallel). Model:'https://schema.org/Number'" .

###  https://smartdatamodels.org/dataModel.Energy/maxInputCurrentParallelAssembly
energy:maxInputCurrentParallelAssembly rdf:type owl:DatatypeProperty ;
                                       rdfs:subPropertyOf :Property ;
                                       rdfs:domain energy:InverterDevice ;
                                       rdfs:range xsd:float ;
                                       rdfs:comment "Property. Max. Current Input with an Parallel Assembly. The unit code (text) is given using the [UN/CEFACT Common Codes](http://wiki.goodrelations-vocabulary.org/Documentation/UN/CEFACT_Common_Codes). For instance, **AMP** represents Ampere. Model:'https://schema.org/Number'. Units:'Ampere'" .

###  https://smartdatamodels.org/dataModel.Energy/nominalPowerAC
energy:nominalPowerAC rdf:type owl:DatatypeProperty ;
                      rdfs:subPropertyOf :Property ;
                      rdfs:domain energy:InverterDevice ;
                      rdfs:range xsd:float ;
                      rdfs:comment "Property. Nominal Power . The unit code (text) is given using the [UN/CEFACT Common Codes](http://wiki.goodrelations-vocabulary.org/Documentation/UN/CEFACT_Common_Codes). For instance, **WTT** represents Watt. Model:'https://schema.org/Number'. Units:'Watt'" .

###  https://smartdatamodels.org/dataModel.Energy/maxOutputPowerAC
energy:maxOutputPowerAC rdf:type owl:DatatypeProperty ;
                        rdfs:subPropertyOf :Property ;
                        rdfs:domain energy:InverterDevice ;
                        rdfs:range xsd:float ;
                        rdfs:comment "Property. Maximum Power or Apparent Power. The unit code (text) is given using the [UN/CEFACT Common Codes](http://wiki.goodrelations-vocabulary.org/Documentation/UN/CEFACT_Common_Codes). For instance, **D46** represents Volt Ampere. Model:'https://schema.org/Number'. Units:'Volt Ampere'" .

###  https://smartdatamodels.org/dataModel.Energy/nominalVoltageAC
energy:nominalVoltageAC rdf:type owl:DatatypeProperty ;
                        rdfs:subPropertyOf :Property ;
                        rdfs:domain energy:InverterDevice ;
                        rdfs:range xsd:float ;
                        rdfs:comment "Property. Nominal battery voltage *(Code U)*. The unit code (text) is given using the [UN/CEFACT Common Codes](http://wiki.goodrelations-vocabulary.org/Documentation/UN/CEFACT_Common_Codes). For instance, **VLT** represents Volt. Model:'https://schema.org/Number'. Units:'Volt'" .

###  https://smartdatamodels.org/dataModel.Energy/nominalAmpereAC
energy:nominalAmpereAC rdf:type owl:DatatypeProperty ;
                       rdfs:subPropertyOf :Property ;
                       rdfs:domain energy:InverterDevice ;
                       rdfs:range xsd:float ;
                       rdfs:comment "Property. Nominal Amperage *(Code I)*. The unit code (text) is given using the [UN/CEFACT Common Codes](http://wiki.goodrelations-vocabulary.org/Documentation/UN/CEFACT_Common_Codes). For instance, **AMP** represents Ampere. Model:'https://schema.org/Number'. Units:'Ampere'" .

###  https://smartdatamodels.org/dataModel.Energy/nominalFrequencyAC
energy:nominalFrequencyAC rdf:type owl:DatatypeProperty ;
                          rdfs:subPropertyOf :Property ;
                          rdfs:domain energy:InverterDevice ;
                          rdfs:range xsd:float ;
                          rdfs:comment "Property. Nominal Frequency. The unit code (text) is given using the [UN/CEFACT Common Codes](http://wiki.goodrelations-vocabulary.org/Documentation/UN/CEFACT_Common_Codes). For instance, **HTZ** represents Hertz. Model:'https://schema.org/Number'. Units:'Hertz'" .

###  https://smartdatamodels.org/dataModel.Energy/powerFactorAC
energy:powerFactorAC rdf:type owl:DatatypeProperty ;
                     rdfs:subPropertyOf :Property ;
                     rdfs:domain energy:InverterDevice ;
                     rdfs:range xsd:float ;
                     rdfs:comment "Property. Power factor for cos phi. A value between [0,1] Units:'Volt'. Model:'http://schema.org/Number'" .

###  https://smartdatamodels.org/dataModel.Energy/euro
energy:euro rdf:type owl:DatatypeProperty ;
            rdfs:domain default:moduleYieldRateType ;
            rdfs:range xsd:float .

###  https://smartdatamodels.org/dataModel.Energy/eta
energy:eta rdf:type owl:DatatypeProperty ;
           rdfs:domain default:moduleYieldRateType ;
           rdfs:range xsd:float .

###  https://smartdatamodels.org/dataModel.Energy/noiseLevel
energy:noiseLevel rdf:type owl:DatatypeProperty ;
                  rdfs:subPropertyOf :Property ;
                  rdfs:domain energy:InverterDevice ;
                  rdfs:range xsd:float ;
                  rdfs:comment "Property. Sound Power level of the Device. The unit code (text) is given using the [UN/CEFACT Common Codes](http://wiki.goodrelations-vocabulary.org/Documentation/UN/CEFACT_Common_Codes). For instance, **2N** represents Decibel. Units:'dB'. Model:'http://schema.org/Number'" .

###  https://smartdatamodels.org/dataModel.Energy/self-consumption
energy:self-consumption rdf:type owl:DatatypeProperty ;
                        rdfs:subPropertyOf :Property ;
                        rdfs:domain energy:InverterDevice ;
                        rdfs:range xsd:float ;
                        rdfs:comment "Property. Self-consumption during nigth. The unit code (text) is given using the [UN/CEFACT Common Codes](http://wiki.goodrelations-vocabulary.org/Documentation/UN/CEFACT_Common_Codes).  For instance, **WTT** represents Watt. Units:'Watt'. Model:'http://schema.org/Number'" .

###  https://smartdatamodels.org/dataModel.Energy/topology
energy:topology rdf:type owl:DatatypeProperty ;
                rdfs:subPropertyOf :Property ;
                rdfs:domain energy:InverterDevice ;
                rdfs:range xsd:string ;
                rdfs:comment "Property. Description of the topology of the installation" .

###  https://smartdatamodels.org/dataModel.Energy/coolingSystem
energy:coolingSystem rdf:type owl:DatatypeProperty ;
                     rdfs:subPropertyOf :Property ;
                     rdfs:domain energy:InverterDevice ;
                     rdfs:range xsd:string ;
                     rdfs:comment "Property.  Cooling System of the Device. Enum:'Convection, OptiCool, Regulated-fan, Other'" .

###  https://smartdatamodels.org/dataModel.Energy/inverterStatus
energy:inverterStatus rdf:type owl:DatatypeProperty ;
                      rdfs:subPropertyOf :Property ;
                      rdfs:domain energy:InverterDevice ;
                      rdfs:range rdf:List ;
                      rdfs:comment "Property. Status of the inverter. A combination of values -- item_type:xsd:string, item_enum:['00-OnSector', '01-PowerFailure/OnBattery', '02-LossCommunication', '03-BatteryFault', '04-SystemShutDown', '05-TensionDip', '06-OverVoltage', '07-VoltageDrop', '08-VoltageIncrease', '09-LineNoise', '10-FrequencyVariation', '11-TransientDistortion', '12-HarmonicDistortion']." .

###  https://smartdatamodels.org/dataModel.Energy/width
energy:width rdf:type owl:DatatypeProperty ;
             rdfs:domain default:internalDimensionType ;
             rdfs:range xsd:float .

###  https://smartdatamodels.org/dataModel.Energy/maximumSystemVoltage
energy:maximumSystemVoltage rdf:type owl:DatatypeProperty ;
                            rdfs:subPropertyOf :Property ;
                            rdfs:domain energy:TechnicalCabinetDevice ;
                            rdfs:range xsd:float ;
                            rdfs:comment "Property. Maximum system voltage permitted for the **module**. The unit code (text) is given using the [UN/CEFACT Common Codes](http://wiki.goodrelations-vocabulary.org/Documentation/UN/CEFACT_Common_Codes). For instance, **VLT** represents Volt" .

###  https://smartdatamodels.org/dataModel.Energy/protectionOthers
energy:protectionOthers rdf:type owl:DatatypeProperty ;
                        rdfs:subPropertyOf :Property ;
                        rdfs:domain energy:TechnicalCabinetDevice ;
                        rdfs:range rdf:List ;
                        rdfs:comment "Property. Others protection of the technical cabinet. A combination of these values. Enum:'abrasion, basement, dampProof, display, doorTearing, dust, forcedOpening, graffiti, insect, other, roofOverload, saltSpray, shielding, solar, vandalism, water' -- item_type:xsd:string, item_enum:['abrasion', 'basement', 'dampProof', 'display', 'doorTearing', 'dust', 'forcedOpening', 'graffiti', 'insect', 'other', 'roofOverload', 'saltSpray', 'shielding', 'solar', 'vandalism', 'water']." .

###  https://smartdatamodels.org/dataModel.Energy/doorCount
energy:doorCount rdf:type owl:DatatypeProperty ;
                 rdfs:subPropertyOf :Property ;
                 rdfs:domain energy:TechnicalCabinetDevice ;
                 rdfs:range xsd:float ;
                 rdfs:comment "Property. Count of doors of the technical Cabinet" .

###  https://smartdatamodels.org/dataModel.Energy/doorType
energy:doorType rdf:type owl:DatatypeProperty ;
                rdfs:subPropertyOf :Property ;
                rdfs:domain energy:TechnicalCabinetDevice ;
                rdfs:range xsd:string ;
                rdfs:comment "Property. Type of door of the technical Cabinet. A unique value of these values. Enum:'mixed, other, solid, transparent'" .

###  https://smartdatamodels.org/dataModel.Energy/doorOpeningAngle
energy:doorOpeningAngle rdf:type owl:DatatypeProperty ;
                        rdfs:subPropertyOf :Property ;
                        rdfs:domain energy:TechnicalCabinetDevice ;
                        rdfs:range xsd:float ;
                        rdfs:comment "Property. Door opening angle expressed in decimal degrees with a range from 0 to 180 degree. The unit code (text) of measurement  is given using the [UN/CEFACT Common Codes](http://wiki.goodrelations-vocabulary.org/Documentation/UN/CEFACT_Common_Codes). For instance, **DD** represents Decimal Degrees" .

###  https://smartdatamodels.org/dataModel.Energy/doorClosingMode
energy:doorClosingMode rdf:type owl:DatatypeProperty ;
                       rdfs:subPropertyOf :Property ;
                       rdfs:domain energy:TechnicalCabinetDevice ;
                       rdfs:range rdf:List ;
                       rdfs:comment "Property. Door closing mode. A unique value of these values. Enum:'fixedHandle, other, revolvingHandle, triangleHandle' -- item_type:xsd:string, item_enum:['fixedHandle', 'other', 'revolvingHandle', 'triangleHandle']." .

###  https://smartdatamodels.org/dataModel.Energy/designMaterials
energy:designMaterials rdf:type owl:DatatypeProperty ;
                       rdfs:subPropertyOf :Property ;
                       rdfs:domain energy:TechnicalCabinetDevice ;
                       rdfs:range rdf:List ;
                       rdfs:comment "Property. Design materials to build the cabinet. A combination of  these values. Enum:'ABS-Plastic, aluminum, fiberGlass, galvanizedSteel, other, polyester, stainlessSteel' -- item_type:xsd:string, item_enum:['ABS-Plastic', 'aluminum', 'fiberGlass', 'galvanizedSteel', 'other', 'polyester', 'stainlessSteel']." .

###  https://smartdatamodels.org/dataModel.Energy/interiorCoating
energy:interiorCoating rdf:type owl:DatatypeProperty ;
                       rdfs:subPropertyOf :Property ;
                       rdfs:domain energy:TechnicalCabinetDevice ;
                       rdfs:range rdf:List ;
                       rdfs:comment "Property. Interior Coating. A combination of these values. Enum:'fiberGlass, heatInsulating, other, plastic, polyester, polyesterResin, steel' -- item_type:xsd:string, item_enum:['fiberGlass', 'heatInsulating', 'other', 'plastic', 'polyester', 'polyesterResin', 'steel']." .

###  https://smartdatamodels.org/dataModel.Energy/exteriorCoating
energy:exteriorCoating rdf:type owl:DatatypeProperty ;
                       rdfs:subPropertyOf :Property ;
                       rdfs:domain energy:TechnicalCabinetDevice ;
                       rdfs:range rdf:List ;
                       rdfs:comment "Property. Interior Coating. A combination of these values. Enum:'fiberGlass, other, plastic, polyester, polyesterResin, steel -- item_type:xsd:string, item_enum:['fiberGlass', 'other', 'plastic', 'polyester', 'polyesterResin', 'steel']." .

###  https://smartdatamodels.org/dataModel.Energy/exteriorFinish
energy:exteriorFinish rdf:type owl:DatatypeProperty ;
                      rdfs:subPropertyOf :Property ;
                      rdfs:domain energy:TechnicalCabinetDevice ;
                      rdfs:range rdf:List ;
                      rdfs:comment "Property. Exterior finish. A combination of these values. Enum:'graffiti, other, raised, roughcast, smooth, textured' -- item_type:xsd:string, item_enum:['graffiti', 'other', 'raised', 'roughcast', 'smooth', 'textured']." .

###  https://smartdatamodels.org/dataModel.Energy/ventilationMode
energy:ventilationMode rdf:type owl:DatatypeProperty ;
                       rdfs:subPropertyOf :Property ;
                       rdfs:domain energy:TechnicalCabinetDevice ;
                       rdfs:range rdf:List ;
                       rdfs:comment "Property. Ventilation mode. A combination of these values. Enum:'airConditioners, dehumidifier, none, other, selfVentilatedGills' -- item_type:xsd:string, item_enum:['airConditioners', 'dehumidifier', 'none', 'other', 'selfVentilatedGills']." .

